Define and prove normal separately

src/ldrfra/WStep.v
@@ -1,4 +1,3 @@
-Require Import Omega.
 Require Import Bool.
 Require Import RelationClasses.
 
@@ -27,26 +26,26 @@ Require Import Mapping.
 
 Require Import PFStep.
 Require Import OrdStep.
-Require Import RelWrites.
+Require Import Writes.
 
 Set Implicit Arguments.
 
 
-Module RelThread.
-  Section RelThread.
+Module WThread.
+  Section WThread.
     Variable lang: language.
     Variable L: Loc.t -> bool.
     Variable ordcr: Ordering.t.
     Variable ordcw: Ordering.t.
 
-    Inductive step rels1: forall (rels2: RelWrites.t) (e: ThreadEvent.t) (e1 e2: Thread.t lang), Prop :=
+    Inductive step rels1: forall (rels2: Writes.t) (e: ThreadEvent.t) (e1 e2: Thread.t lang), Prop :=
     | step_intro
         pf e e1 e2
         (STEP: @OrdThread.step lang L ordcr ordcw pf e e1 e2):
-        step rels1 (RelWrites.append L e rels1) e e1 e2
+        step rels1 (Writes.append L e rels1) e e1 e2
     .
 
-    Inductive steps rels1: forall (rels2: RelWrites.t) (e1 e2: Thread.t lang), Prop :=
+    Inductive steps rels1: forall (rels2: Writes.t) (e1 e2: Thread.t lang), Prop :=
     | steps_refl
         e:
         steps rels1 rels1 e e
@@ -58,7 +57,7 @@ Module RelThread.
     .
     Hint Constructors steps.
 
-    Inductive tau_steps rels1: forall (rels2: RelWrites.t) (e1 e2: Thread.t lang), Prop :=
+    Inductive tau_steps rels1: forall (rels2: Writes.t) (e1 e2: Thread.t lang), Prop :=
     | tau_steps_refl
         e:
         tau_steps rels1 rels1 e e
@@ -71,7 +70,7 @@ Module RelThread.
     .
     Hint Constructors tau_steps.
 
-    Inductive opt_step rels1: forall (rels2: RelWrites.t) (e: ThreadEvent.t) (e1 e2: Thread.t lang), Prop :=
+    Inductive opt_step rels1: forall (rels2: Writes.t) (e: ThreadEvent.t) (e1 e2: Thread.t lang), Prop :=
     | step_none
         e:
         opt_step rels1 rels1 ThreadEvent.silent e e
@@ -118,7 +117,7 @@ Module RelThread.
           tau_steps rels1 rels2 e1 e2.
     Proof.
       induction STEPS; eauto. inv H. inv TSTEP. i.
-      specialize (IHSTEPS (RelWrites.append L e rels1)). des.
+      specialize (IHSTEPS (Writes.append L e rels1)). des.
       esplits. econs 2; eauto. econs; eauto.
     Qed.
 
@@ -139,7 +138,7 @@ Module RelThread.
       inv H. inv STEP; [|inv STEP0; inv LOCAL].
       econs 2; eauto.
       - replace rels with
-            (RelWrites.append
+            (Writes.append
                L (ThreadEvent.promise loc from to Message.reserve Memory.op_kind_add) rels)
             at 2 by ss.
         econs. econs 1; eauto.
@@ -156,7 +155,7 @@ Module RelThread.
       inv H. inv STEP; [|inv STEP0; inv LOCAL].
       econs 2; eauto.
       - replace rels with
-            (RelWrites.append
+            (Writes.append
                L (ThreadEvent.promise loc from to Message.reserve Memory.op_kind_cancel) rels)
             at 2 by ss.
         econs. econs 1; eauto.
@@ -286,54 +285,54 @@ Module RelThread.
     Qed.
 
 
-    (* RelWrites.wf *)
+    (* Writes.wf *)
 
-    Lemma step_rels_wf
+    Lemma step_writes_wf
           rels1 rels2 e e1 e2
-          (RELS1: RelWrites.wf rels1 (Local.promises (Thread.local e1)) (Thread.memory e1))
+          (RELS1: Writes.wf rels1 (Local.promises (Thread.local e1)) (Thread.memory e1))
           (STEP: step rels1 rels2 e e1 e2):
-      RelWrites.wf rels2 (Local.promises (Thread.local e2)) (Thread.memory e2).
+      Writes.wf rels2 (Local.promises (Thread.local e2)) (Thread.memory e2).
     Proof.
-      inv STEP. eauto using RelWrites.step_wf.
+      inv STEP. eauto using Writes.step_wf.
     Qed.
 
-    Lemma steps_rels_wf
+    Lemma steps_writes_wf
           rels1 rels2 e1 e2
-          (RELS1: RelWrites.wf rels1 (Local.promises (Thread.local e1)) (Thread.memory e1))
+          (RELS1: Writes.wf rels1 (Local.promises (Thread.local e1)) (Thread.memory e1))
           (STEPS: steps rels1 rels2 e1 e2):
-      RelWrites.wf rels2 (Local.promises (Thread.local e2)) (Thread.memory e2).
+      Writes.wf rels2 (Local.promises (Thread.local e2)) (Thread.memory e2).
     Proof.
       induction STEPS; eauto.
-      apply IHSTEPS. eapply step_rels_wf; eauto.
+      apply IHSTEPS. eapply step_writes_wf; eauto.
     Qed.
 
     Lemma step_rels_disjoint
           rels1 rels2 e e1 e2 promises
-          (RELS1: RelWrites.wf rels1 (Local.promises (Thread.local e1)) (Thread.memory e1))
+          (RELS1: Writes.wf rels1 (Local.promises (Thread.local e1)) (Thread.memory e1))
           (STEP: step rels1 rels2 e e1 e2)
           (DISJOINT: Memory.disjoint (Local.promises (Thread.local e1)) promises)
           (LE: Memory.le promises (Thread.memory e1))
-          (RELS: RelWrites.wf rels1 promises (Thread.memory e1)):
-      RelWrites.wf rels2 promises (Thread.memory e2).
+          (RELS: Writes.wf rels1 promises (Thread.memory e1)):
+      Writes.wf rels2 promises (Thread.memory e2).
     Proof.
-      inv STEP. eauto using RelWrites.step_disjoint.
+      inv STEP. eauto using Writes.step_disjoint.
     Qed.
 
     Lemma steps_rels_disjoint
           rels1 rels2 e1 e2 lc
-          (RELS1: RelWrites.wf rels1 (Local.promises (Thread.local e1)) (Thread.memory e1))
+          (RELS1: Writes.wf rels1 (Local.promises (Thread.local e1)) (Thread.memory e1))
           (STEPS: steps rels1 rels2 e1 e2)
           (WF1: Local.wf (Thread.local e1) (Thread.memory e1))
           (SC1: Memory.closed_timemap (Thread.sc e1) (Thread.memory e1))
           (CLOSED1: Memory.closed (Thread.memory e1))
           (DISJOINT: Local.disjoint (Thread.local e1) lc)
           (WF: Local.wf lc (Thread.memory e1))
-          (RELS: RelWrites.wf rels1 (Local.promises lc) (Thread.memory e1)):
-      RelWrites.wf rels2 (Local.promises lc) (Thread.memory e2).
+          (RELS: Writes.wf rels1 (Local.promises lc) (Thread.memory e1)):
+      Writes.wf rels2 (Local.promises lc) (Thread.memory e2).
     Proof.
       induction STEPS; ss.
       hexploit step_rels_disjoint; eauto; try apply DISJOINT; try apply WF. i.
-      hexploit step_rels_wf; eauto. i.
+      hexploit step_writes_wf; eauto. i.
       inv STEP.
       exploit OrdThread.step_future; eauto. i. des.
       exploit OrdThread.step_disjoint; eauto. i. des.
@@ -361,8 +360,8 @@ Module RelThread.
       exploit OrdThread.step_future; try apply STEP; eauto. i. des.
       exploit OrdThread.step_future; try apply STEP0; eauto. i. des.
       exploit IHSTEPS; eauto. i. des. exists fe2. splits; eauto.
-      replace (RelWrites.append L e rels1) with (RelWrites.append L fe rels1) in STEPS0; cycle 1.
-      { unfold RelWrites.append. destruct e; inv EVENT; ss.
+      replace (Writes.append L e rels1) with (Writes.append L fe rels1) in STEPS0; cycle 1.
+      { unfold Writes.append. destruct e; inv EVENT; ss.
         - inv FROM. inv TO. refl.
         - inv FROM. inv TO. refl.
         - inv FROM. inv TO. refl.
@@ -379,10 +378,10 @@ Module RelThread.
           (CAP: Memory.cap (Thread.memory e1) mem1)
           (SC_MAX: Memory.max_concrete_timemap mem1 sc1)
           (STEPS: tau_steps rels1 rels2 (Thread.mk lang (Thread.state e1) (Thread.local e1) sc1 mem1) e2)
-          (STEP: RelThread.step rels2 rels3 e e2 e3):
+          (STEP: WThread.step rels2 rels3 e e2 e3):
         exists rels3' e' e2' e3',
           (<<STEPS: tau_steps rels1 rels2 e1 e2'>>) /\
-          (<<STEP: RelThread.step rels2 rels3' e' e2' e3'>>) /\
+          (<<STEP: WThread.step rels2 rels3' e' e2' e3'>>) /\
           (<<LOCAL: local_map ident_map (Thread.local e2) (Thread.local e2')>>) /\
           (<<EVENT: tevent_map ident_map e' e>>).
     Proof.
@@ -659,7 +658,7 @@ Module RelThread.
           (STEP: step rels1 rels2 e e1 e2):
       rels2 = rels1 \/ exists a, rels2 = a :: rels1.
     Proof.
-      inv STEP. unfold RelWrites.append. des_ifs; eauto.
+      inv STEP. unfold Writes.append. des_ifs; eauto.
     Qed.
 
     (* Lemma step_non_concrete *)
@@ -754,23 +753,23 @@ Module RelThread.
     (*   inv H. inv STEP; inv STEP0; inv LOCAL. inv PROMISE; ss. *)
     (*   revert GET. erewrite Memory.remove_o; eauto. condtac; ss; eauto. *)
     (* Qed. *)
-  End RelThread.
-End RelThread.
+  End WThread.
+End WThread.
 
 
-Module RelConfiguration.
-  Section RelConfiguration.
+Module WConfiguration.
+  Section WConfiguration.
     Variable L: Loc.t -> bool.
     Variable ordcr ordcw: Ordering.t.
 
     Inductive step:
-      forall (e: ThreadEvent.t) (tid: Ident.t) (rels1 rels2: RelWrites.t) (c1 c2: Configuration.t), Prop :=
+      forall (e: ThreadEvent.t) (tid: Ident.t) (rels1 rels2: Writes.t) (c1 c2: Configuration.t), Prop :=
     | step_intro
         rels1 rels2
         e tid c1 lang st1 lc1 e2 e3 st4 lc4 sc4 memory4
         (TID: IdentMap.find tid (Configuration.threads c1) = Some (existT _ lang st1, lc1))
         (CANCELS: rtc (@Thread.cancel_step _) (Thread.mk _ st1 lc1 (Configuration.sc c1) (Configuration.memory c1)) e2)
-        (STEP: RelThread.opt_step L ordcr ordcw rels1 rels2 e e2 e3)
+        (STEP: WThread.opt_step L ordcr ordcw rels1 rels2 e e2 e3)
         (RESERVES: rtc (@Thread.reserve_step _) e3 (Thread.mk _ st4 lc4 sc4 memory4))
         (CONSISTENT: ThreadEvent.get_machine_event e <> MachineEvent.failure ->
                      OrdThread.consistent L ordcr ordcw (Thread.mk _ st4 lc4 sc4 memory4)):
@@ -778,7 +777,7 @@ Module RelConfiguration.
              c1 (Configuration.mk (IdentMap.add tid (existT _ _ st4, lc4) (Configuration.threads c1)) sc4 memory4)
     .
 
-    Inductive steps rels1: forall (rels2: RelWrites.t) (c1 c2: Configuration.t), Prop :=
+    Inductive steps rels1: forall (rels2: Writes.t) (c1 c2: Configuration.t), Prop :=
     | steps_refl
         c:
         steps rels1 rels1 c c
@@ -827,21 +826,21 @@ Module RelConfiguration.
       inv WF1. inv WF. inv STEP; s.
       exploit THREADS; eauto. i.
       exploit Thread.rtc_cancel_step_future; try exact CANCELS; eauto. s. i. des.
-      exploit RelThread.opt_step_future; try exact STEP0; eauto. i. des.
+      exploit WThread.opt_step_future; try exact STEP0; eauto. i. des.
       exploit Thread.rtc_reserve_step_future; try exact RESERVES; eauto. s. i. des.
       econs; ss. econs.
       - i. Configuration.simplify.
         + exploit THREADS; try apply TH1; eauto. i.
           exploit Thread.rtc_tau_step_disjoint; try eapply rtc_implies;
             try eapply Thread.cancel_step_tau_step; try exact CANCELS; eauto. i. des.
-          exploit RelThread.opt_step_disjoint; try exact STEP0; eauto. i. des.
+          exploit WThread.opt_step_disjoint; try exact STEP0; eauto. i. des.
           exploit Thread.rtc_tau_step_disjoint; try eapply rtc_implies;
             try eapply Thread.reserve_step_tau_step; try exact RESERVES; eauto. s. i. des.
           symmetry. ss.
         + exploit THREADS; try apply TH1; eauto. i.
           exploit Thread.rtc_tau_step_disjoint; try eapply rtc_implies;
             try eapply Thread.cancel_step_tau_step; try exact CANCELS; eauto. i. des.
-          exploit RelThread.opt_step_disjoint; try exact STEP0; eauto. i. des.
+          exploit WThread.opt_step_disjoint; try exact STEP0; eauto. i. des.
           exploit Thread.rtc_tau_step_disjoint; try eapply rtc_implies;
             try eapply Thread.reserve_step_tau_step; try exact RESERVES; eauto. s. i. des.
           ss.
@@ -850,7 +849,7 @@ Module RelConfiguration.
         exploit THREADS; try apply TH; eauto. i. exploit THREADS; try apply TH1; eauto. i.
         exploit Thread.rtc_tau_step_disjoint; try eapply rtc_implies;
           try eapply Thread.cancel_step_tau_step; try exact CANCELS; eauto. i. des.
-        exploit RelThread.opt_step_disjoint; try exact STEP0; eauto. i. des.
+        exploit WThread.opt_step_disjoint; try exact STEP0; eauto. i. des.
         exploit Thread.rtc_tau_step_disjoint; try eapply rtc_implies;
           try eapply Thread.reserve_step_tau_step; try exact RESERVES; eauto. s. i. des.
         ss.
@@ -868,7 +867,7 @@ Module RelConfiguration.
       inv STEP. s.
       inv WF1. inv WF. exploit THREADS; eauto. i. clear DISJOINT THREADS.
       exploit Thread.rtc_cancel_step_future; eauto. s. i. des.
-      exploit RelThread.opt_step_future; eauto. i. des.
+      exploit WThread.opt_step_future; eauto. i. des.
       exploit Thread.rtc_reserve_step_future; eauto. s. i. des.
       splits; (etrans; [etrans|]; eauto).
     Qed.
@@ -913,19 +912,19 @@ Module RelConfiguration.
     (*   split; cycle 1. *)
     (*   { inv STEP. inv STEP0; inv STEP; inv LOCAL; ss. *)
     (*     - inv LOCAL0. inv STEP. exploit Memory.write_get2; eauto. i. des. *)
-    (*       exploit RelThread.reserve_steps_get_None; eauto. i. des. inv WRITE. ss. *)
+    (*       exploit WThread.reserve_steps_get_None; eauto. i. des. inv WRITE. ss. *)
     (*     - inv LOCAL1. inv STEP. inv LOCAL2. inv STEP. *)
     (*       exploit Memory.write_get2; eauto. i. des. *)
-    (*       exploit RelThread.reserve_steps_get_None; eauto. i. des. inv WRITE. ss. *)
+    (*       exploit WThread.reserve_steps_get_None; eauto. i. des. inv WRITE. ss. *)
     (*   } *)
     (*   ii. revert FIND. rewrite IdentMap.gsspec. condtac; ss. *)
     (*   { i. inv FIND. *)
     (*     inv STEP. inv STEP0; inv STEP; inv LOCAL; ss. *)
     (*     - inv LOCAL0. inv STEP. exploit Memory.write_get2; eauto. i. des. *)
-    (*       exploit RelThread.reserve_steps_get_None; eauto. i. des. inv WRITE. ss. *)
+    (*       exploit WThread.reserve_steps_get_None; eauto. i. des. inv WRITE. ss. *)
     (*     - inv LOCAL1. inv STEP. inv LOCAL2. inv STEP. *)
     (*       exploit Memory.write_get2; eauto. i. des. *)
-    (*       exploit RelThread.reserve_steps_get_None; eauto. i. des. inv WRITE. ss. *)
+    (*       exploit WThread.reserve_steps_get_None; eauto. i. des. inv WRITE. ss. *)
     (*   } *)
 
     (*   i. inv WF1. inv WF. hexploit DISJOINT; eauto. i. *)
@@ -935,7 +934,7 @@ Module RelConfiguration.
     (*     try eapply Thread.cancel_step_tau_step; try exact CANCELS; eauto. i. des. *)
     (*   exploit Thread.rtc_tau_step_future; try eapply rtc_implies; *)
     (*     try eapply Thread.cancel_step_tau_step; try exact CANCELS; eauto. s. i. des. *)
-    (*   exploit RelThread.step_future; try exact STEP; eauto. i. des. *)
+    (*   exploit WThread.step_future; try exact STEP; eauto. i. des. *)
     (*   inv STEP. inv STEP0; inv STEP; inv LOCAL; inv WRITE; ss. *)
     (*   - inv LOCAL0. inv STEP. inv WRITE. *)
     (*     exploit Memory.promise_disjoint; try eapply WF; try eapply DISJOINT2; eauto. i. des. *)
@@ -975,9 +974,9 @@ Module RelConfiguration.
     (* Proof. *)
     (*   inv STEP. ss. *)
     (*   exploit PROMISES1; eauto. i. *)
-    (*   exploit RelThread.cancel_steps_get_None; eauto. i. des. *)
-    (*   exploit RelThread.opt_step_get_None; eauto. i. des. *)
-    (*   exploit RelThread.reserve_steps_get_None; eauto. i. des. *)
+    (*   exploit WThread.cancel_steps_get_None; eauto. i. des. *)
+    (*   exploit WThread.opt_step_get_None; eauto. i. des. *)
+    (*   exploit WThread.reserve_steps_get_None; eauto. i. des. *)
     (*   splits; eauto. i. *)
     (*   revert FIND. rewrite IdentMap.gsspec. condtac; eauto. i. inv FIND. ss. *)
     (* Qed. *)
@@ -997,7 +996,7 @@ Module RelConfiguration.
     (*   exploit step_get_None; eauto. i. des. *)
     (*   eapply IHSTEPS; eauto. *)
     (*   ii. inv STEP. ss. inv STEP0; ss. inv STEP. *)
-    (*   unfold RelWrites.append in H. des_ifs. inv H; ss. inv H0. *)
+    (*   unfold Writes.append in H. des_ifs. inv H; ss. inv H0. *)
     (*   eapply EVENT; eauto. *)
     (* Qed. *)
 
@@ -1007,23 +1006,23 @@ Module RelConfiguration.
     (*       (WF1: Configuration.wf c1) *)
     (*       (RELS1: forall tid lang st lc *)
     (*                 (TH: IdentMap.find tid (Configuration.threads c1) = Some (existT _ lang st, lc)), *)
-    (*           RelWrites.wf rels1 (Local.promises lc) (Configuration.memory c1)) *)
+    (*           Writes.wf rels1 (Local.promises lc) (Configuration.memory c1)) *)
     (*       (STEP: step e tid rels1 rels2 c1 c2) *)
     (*       (WRITE: ThreadEvent.is_writing e = Some (loc, from, to, val, released, ord)): *)
     (*   ~ List.In (loc, to) rels1. *)
     (* Proof. *)
     (*   ii. inv STEP. inv STEP0; ss. *)
     (*   hexploit RELS1; eauto. i. *)
-    (*   hexploit (@RelThread.steps_rels_wf lang L ordcr ordcw); *)
-    (*     try eapply RelThread.tau_steps_steps; *)
-    (*     try eapply RelThread.cancel_steps_tau_steps; eauto; ss; eauto. i. *)
+    (*   hexploit (@WThread.steps_writes_wf lang L ordcr ordcw); *)
+    (*     try eapply WThread.tau_steps_steps; *)
+    (*     try eapply WThread.cancel_steps_tau_steps; eauto; ss; eauto. i. *)
     (*   inv STEP. inv STEP0; inv STEP; inv LOCAL; ss. *)
     (*   - inv LOCAL0. inv STEP. inv WRITE0. *)
-    (*     exploit RelThread.promise_rels_wf; eauto. i. des. *)
+    (*     exploit WThread.promise_writes_wf; eauto. i. des. *)
     (*     exploit Memory.promise_get0; eauto; try by (inv PROMISE; ss). i. des. *)
     (*     congr. *)
     (*   - inv LOCAL1. inv STEP. inv LOCAL2. inv STEP. inv WRITE0. ss. *)
-    (*     exploit RelThread.promise_rels_wf; eauto. i. des. *)
+    (*     exploit WThread.promise_writes_wf; eauto. i. des. *)
     (*     exploit Memory.promise_get0; eauto; try by (inv PROMISE; ss). i. des. *)
     (*     congr. *)
     (* Qed. *)
@@ -1034,7 +1033,7 @@ Module RelConfiguration.
     (* Definition reserve_only (c: Configuration.t): Prop := *)
     (*   forall tid lang st lc *)
     (*     (FIND: IdentMap.find tid (Configuration.threads c) = Some (existT _ lang st, lc)), *)
-    (*     RelThread.reserve_only L (Local.promises lc). *)
+    (*     WThread.reserve_only L (Local.promises lc). *)
 
     (* Lemma init_reserve_only s: *)
     (*   reserve_only (Configuration.init s). *)
@@ -1058,9 +1057,9 @@ Module RelConfiguration.
     (*   inv FIND. apply inj_pair2 in H1. subst. *)
     (*   unfold reserve_only in RESERVE. *)
     (*   hexploit RESERVE; eauto. i. *)
-    (*   hexploit RelThread.cancel_steps_reserve_only; try exact CANCELS; eauto. i. des. *)
-    (*   hexploit RelThread.opt_step_reserve_only; try exact STEP0; eauto. i. *)
-    (*   hexploit RelThread.reserve_steps_reserve_only; try exact RESERVES; eauto. *)
+    (*   hexploit WThread.cancel_steps_reserve_only; try exact CANCELS; eauto. i. des. *)
+    (*   hexploit WThread.opt_step_reserve_only; try exact STEP0; eauto. i. *)
+    (*   hexploit WThread.reserve_steps_reserve_only; try exact RESERVES; eauto. *)
     (* Qed. *)
 
     (* Lemma steps_reserve_only *)
@@ -1079,7 +1078,7 @@ Module RelConfiguration.
     (*   rels2 = rels1 \/ exists a, rels2 = a :: rels1. *)
     (* Proof. *)
     (*   inv STEP. inv STEP0; eauto. inv STEP. *)
-    (*   unfold RelWrites.append. des_ifs; eauto. *)
+    (*   unfold Writes.append. des_ifs; eauto. *)
     (* Qed. *)
 
     (* Lemma steps_rels_incl *)
@@ -1106,48 +1105,66 @@ Module RelConfiguration.
     (*       msg = Message.reserve>>. *)
     (* Proof. *)
     (*   inv STEP. ss. *)
-    (*   hexploit RelThread.cancel_steps_non_concrete; eauto. i. des. *)
-    (*   hexploit RelThread.opt_step_non_concrete; eauto. i. des. *)
-    (*   hexploit RelThread.reserve_steps_non_concrete; eauto. *)
+    (*   hexploit WThread.cancel_steps_non_concrete; eauto. i. des. *)
+    (*   hexploit WThread.opt_step_non_concrete; eauto. i. des. *)
+    (*   hexploit WThread.reserve_steps_non_concrete; eauto. *)
     (* Qed. *)
-  End RelConfiguration.
-End RelConfiguration.
+  End WConfiguration.
+End WConfiguration.
 
 
-Module RelRARace.
-  Section RelRARace.
+Module RARaceW.
+  Section RARaceW.
     Variable L: Loc.t -> bool.
     Variable ordcr ordcw: Ordering.t.
 
-    Definition ra_race (rels: RelWrites.t) (tview: TView.t) (loc: Loc.t) (to: Time.t) (ordr: Ordering.t): Prop :=
-      (<<LOC: L loc>>) /\
-      (<<HIGHER: Time.lt ((View.rlx (TView.cur tview)) loc) to>>) /\
-      ((<<ORDW: ~ List.In (loc, to) rels>>) \/
-       (<<ORDR: Ordering.le ordr Ordering.strong_relaxed>>)).
+    Definition wr_race (rels: Writes.t) (tview: TView.t) (loc: Loc.t) (to: Time.t) (ord: Ordering.t): Prop :=
+      exists ordw,
+        (<<LOC: L loc>>) /\
+        (<<HIGHER: Time.lt ((View.rlx (TView.cur tview)) loc) to>>) /\
+        (<<IN: List.In (loc, to, ordw) rels>>) /\
+        ((<<ORDW: Ordering.le ordw Ordering.strong_relaxed>>) \/
+         (<<ORDR: Ordering.le ord Ordering.strong_relaxed>>)).
 
-    Definition ra_race_steps (rels: RelWrites.t) (c: Configuration.t): Prop :=
+    Definition ww_race (rels: Writes.t) (tview: TView.t) (loc: Loc.t) (to: Time.t) (ord: Ordering.t): Prop :=
+      exists ordw,
+        (<<LOC: L loc>>) /\
+        (<<HIGHER: Time.lt ((View.rlx (TView.cur tview)) loc) to>>) /\
+        (<<IN: List.In (loc, to, ordw) rels>>) /\
+        ((<<ORDW1: Ordering.le ordw Ordering.na>>) \/
+         (<<ORDW2: Ordering.le ord Ordering.na>>)).
+
+    Definition ra_race_steps (rels: Writes.t) (c: Configuration.t): Prop :=
       exists tid rels2 rels3 rels4
-        c2 lang st2 lc2 e loc to val released ord e3 e4,
-        (<<STEPS: RelConfiguration.steps L ordcr ordcw rels rels2 c c2>>) /\
+        c2 lang st2 lc2 e loc to ord e3 e4,
+        (<<STEPS: WConfiguration.steps L ordcr ordcw rels rels2 c c2>>) /\
         (<<TID: IdentMap.find tid (Configuration.threads c2) = Some (existT _ lang st2, lc2)>>) /\
-        (<<THREAD_STEPS: RelThread.steps L ordcr ordcw rels2 rels3
+        (<<THREAD_STEPS: WThread.steps L ordcr ordcw rels2 rels3
                                          (Thread.mk _ st2 lc2 (Configuration.sc c2) (Configuration.memory c2)) e3>>) /\
         (<<CONS: Local.promise_consistent (Thread.local e3)>>) /\
-        (<<THREAD_STEP: RelThread.step L ordcr ordcw rels3 rels4 e e3 e4>>) /\
-        (<<READ: ThreadEvent.is_reading e = Some (loc, to, val, released, ord)>>) /\
-        (<<RARACE: ra_race rels3 (Local.tview (Thread.local e3)) loc to ord>>).
+        (<<THREAD_STEP: WThread.step L ordcr ordcw rels3 rels4 e e3 e4>>) /\
+        (<<RARACE: (exists val released,
+                       (<<READ: ThreadEvent.is_reading e = Some (loc, to, val, released, ord)>>) /\
+                       (<<WRRACE: wr_race rels3 (Local.tview (Thread.local e3)) loc to ord>>)) \/
+                   (exists from to' val released,
+                       (<<WRITE: ThreadEvent.is_writing e = Some (loc, from, to', val, released, ord)>>) /\
+                       (<<WWRACE: ww_race rels3 (Local.tview (Thread.local e3)) loc to ord>>))>>).
 
-    Definition racefree (rels: RelWrites.t) (c: Configuration.t): Prop :=
+    Definition racefree (rels: Writes.t) (c: Configuration.t): Prop :=
       forall tid rels2 rels3 rels4
-        c2 lang st2 lc2 e loc to val released ord e3 e4
-        (STEPS: RelConfiguration.steps L ordcr ordcw rels rels2 c c2)
+        c2 lang st2 lc2 e loc to ord e3 e4
+        (STEPS: WConfiguration.steps L ordcr ordcw rels rels2 c c2)
         (TID: IdentMap.find tid (Configuration.threads c2) = Some (existT _ lang st2, lc2))
-        (THREAD_STEPS: RelThread.steps L ordcr ordcw rels2 rels3
+        (THREAD_STEPS: WThread.steps L ordcr ordcw rels2 rels3
                                        (Thread.mk _ st2 lc2 (Configuration.sc c2) (Configuration.memory c2)) e3)
         (CONS: Local.promise_consistent (Thread.local e3))
-        (THREAD_STEP: RelThread.step L ordcr ordcw rels3 rels4 e e3 e4)
-        (READ: ThreadEvent.is_reading e = Some (loc, to, val, released, ord))
-        (RARACE: ra_race rels3 (Local.tview (Thread.local e3)) loc to ord),
+        (THREAD_STEP: WThread.step L ordcr ordcw rels3 rels4 e e3 e4)
+        (RARACE: (exists val released,
+                     (<<READ: ThreadEvent.is_reading e = Some (loc, to, val, released, ord)>>) /\
+                     (<<WRRACE: wr_race rels3 (Local.tview (Thread.local e3)) loc to ord>>)) \/
+                 (exists from to' val released,
+                     (<<WRITE: ThreadEvent.is_writing e = Some (loc, from, to', val, released, ord)>>) /\
+                     (<<WWRACE: ww_race rels3 (Local.tview (Thread.local e3)) loc to ord>>))),
         False.
 
     Definition racefree_syn (syn: Threads.syntax): Prop :=
@@ -1156,7 +1173,7 @@ Module RelRARace.
     Lemma step_racefree
           e tid rels1 rels2 c1 c2
           (RACEFREE: racefree rels1 c1)
-          (STEP: RelConfiguration.step L ordcr ordcw e tid rels1 rels2 c1 c2):
+          (STEP: WConfiguration.step L ordcr ordcw e tid rels1 rels2 c1 c2):
       racefree rels2 c2.
     Proof.
       ii. eapply RACEFREE; eauto. econs 2; eauto.
@@ -1164,12 +1181,12 @@ Module RelRARace.
 
     Lemma step_ord_step
           e tid rels1 rels2 c1 c2
-          (STEP: RelConfiguration.step L ordcr ordcw e tid rels1 rels2 c1 c2):
+          (STEP: WConfiguration.step L ordcr ordcw e tid rels1 rels2 c1 c2):
       OrdConfiguration.step L ordcr ordcw e tid c1 c2.
     Proof.
       inv STEP. econs; eauto. inv STEP0.
       - econs 1.
       - inv STEP. econs 2. eauto.
     Qed.
-  End RelRARace.
-End RelRARace.
+  End RARaceW.
+End RARaceW.
