src/ldrfra/Stable.v
@@ -21,13 +21,14 @@ Require Import TView.
 Require Import Local.
 Require Import Thread.
 
-Require Import RAStep.
+Require Import OrdStep.
+Require Import Writes.
 
 Set Implicit Arguments.
 
 
-Module Stable.
-  Section Stable.
+Module Normal.
+  Section Normal.
     Variable L: Loc.t -> bool.
 
     (* normal *)
@@ -83,1233 +84,1491 @@ Module Stable.
       - apply singleton_rw_normal_view. ss.
     Qed.
 
-
-    (* stable *)
-
-    Definition stable_view (mem: Memory.t) (view: View.t): Prop :=
-      forall loc from val released
-        (LOC: L loc)
-        (GET: Memory.get loc ((View.rlx view) loc) mem =
-              Some (from, Message.concrete val (Some released))),
-        View.le released view.
-
-    Definition stable_timemap (mem: Memory.t) (tm: TimeMap.t): Prop :=
-      stable_view mem (View.mk tm tm).
-
-    Inductive stable_tview (mem: Memory.t) (tview: TView.t): Prop :=
-    | stable_tview_intro
-        (REL: forall loc (LOC: ~ L loc), stable_view mem ((TView.rel tview) loc))
-        (CUR: stable_view mem (TView.cur tview))
-        (ACQ: stable_view mem (TView.acq tview))
-    .
-
-    Definition stable_memory (rels: RelWrites.t) (mem: Memory.t): Prop :=
-      forall loc from to val released
-        (LOC: ~ L loc \/ List.In (loc, to) rels)
-        (GET: Memory.get loc to mem = Some (from, Message.concrete val (Some released))),
-        stable_view mem released.
-
-
-    Lemma future_stable_view
-          mem1 mem2 view
-          (CLOSED: Memory.closed_view view mem1)
-          (STABLE: stable_view mem1 view)
-          (MEM_FUTURE: Memory.future mem1 mem2):
-      stable_view mem2 view.
+    Lemma get_normal_view
+          mem loc from to val released
+          (MEM: normal_memory mem)
+          (GET: Memory.get loc to mem = Some (from, Message.concrete val released)):
+      normal_view (View.unwrap released).
     Proof.
-      ii. inv CLOSED. specialize (RLX loc). des.
-      exploit Memory.future_get1; try exact RLX; eauto. i. des.
-      rewrite GET0 in *. inv GET. inv MSG_LE. inv RELEASED.
-      exploit STABLE; eauto.
+      destruct released; ss. eapply MEM; eauto.
     Qed.
-
-    Lemma future_stable_tview
-          mem1 mem2 tview
-          (CLOSED: TView.closed tview mem1)
-          (STABLE: stable_tview mem1 tview)
-          (MEM_FUTURE: Memory.future mem1 mem2):
-      stable_tview mem2 tview.
-    Proof.
-      destruct tview. inv CLOSED. inv STABLE. ss.
-      econs; ss; eauto using future_stable_view.
-    Qed.
-
-    Lemma join_stable_view
-          mem view1 view2
-          (STABLE1: stable_view mem view1)
-          (STABLE2: stable_view mem view2):
-      stable_view mem (View.join view1 view2).
-    Proof.
-      ii. unfold stable_view in *.
-      unfold View.join, TimeMap.join in GET. ss.
-      exploit Time.join_cases. i. des.
-      - erewrite x0 in GET.
-        exploit STABLE1; eauto. i.
-        etrans; eauto. apply View.join_l.
-      - erewrite x0 in GET.
-        exploit STABLE2; eauto. i.
-        etrans; eauto. apply View.join_r.
-    Qed.
-
-    Lemma bot_stable_view
-          mem
-          (MEM: Memory.closed mem):
-      stable_view mem View.bot.
-    Proof.
-      ii. inv MEM. rewrite INHABITED in *. inv GET.
-    Qed.
-
-    Lemma singleton_ur_stable_view
-          mem loc ts
-          (MEM: Memory.closed mem)
-          (LOC: ~ L loc):
-      stable_view mem (View.singleton_ur loc ts).
-    Proof.
-      ii. revert GET. ss.
-      unfold TimeMap.singleton, LocFun.add, LocFun.init, LocFun.find.
-      condtac; subst; ss. i.
-      inv MEM. rewrite INHABITED in *. inv GET.
-    Qed.
-
-    Lemma singleton_rw_stable_view
-          mem loc ts
-          (MEM: Memory.closed mem)
-          (LOC: ~ L loc):
-      stable_view mem (View.singleton_rw loc ts).
-    Proof.
-      ii. revert GET. ss.
-      unfold TimeMap.singleton, LocFun.add, LocFun.init, LocFun.find.
-      condtac; subst; ss. i.
-      inv MEM. rewrite INHABITED in *. inv GET.
-    Qed.
-
-    Lemma singleton_ur_if_stable_view
-          mem b loc ts
-          (MEM: Memory.closed mem)
-          (LOC: ~ L loc):
-      stable_view mem (View.singleton_ur_if b loc ts).
-    Proof.
-      unfold View.singleton_ur_if. condtac.
-      - apply singleton_ur_stable_view; ss.
-      - apply singleton_rw_stable_view; ss.
-    Qed.
-
-    Lemma stable_view_stable_timemap
-          mem view
-          (VIEW: View.wf view)
-          (STABLE: stable_view mem view):
-      stable_timemap mem (View.rlx view).
-    Proof.
-      ii. etrans; [eapply STABLE|]; eauto.
-      econs; ss; try refl. apply VIEW.
-    Qed.
-
-    Lemma join_stable_timemap
-          mem tm1 tm2
-          (STABLE1: stable_timemap mem tm1)
-          (STABLE2: stable_timemap mem tm2):
-      stable_timemap mem (TimeMap.join tm1 tm2).
-    Proof.
-      unfold stable_timemap in *.
-      hexploit join_stable_view; [exact STABLE1|exact STABLE2|]. ss.
-    Qed.
-
-    Lemma stable_tview_read_tview
-          mem tview
-          loc from val released ord
-          (WF: TView.wf tview)
-          (NORMAL: normal_tview tview)
-          (STABLE: stable_tview mem tview)
-          (LOC: L loc)
-          (GET: Memory.get loc ((View.rlx (TView.cur tview)) loc) mem =
-                Some (from, Message.concrete val released)):
-      TView.read_tview tview loc ((View.rlx (TView.cur tview)) loc) released ord = tview.
-    Proof.
-      inv STABLE. inv NORMAL.
-      destruct tview. unfold TView.read_tview. ss. f_equal.
-      - rewrite (@View.le_join_l cur); cycle 1.
-        { unfold View.singleton_ur_if. condtac; ss.
-          - unfold View.singleton_ur. econs; ss.
-            + ii. unfold TimeMap.singleton, LocFun.add, LocFun.find, LocFun.init.
-              condtac; try apply Time.bot_spec. subst.
-              rewrite CUR0; ss. refl.
-            + ii. unfold TimeMap.singleton, LocFun.add, LocFun.find, LocFun.init.
-              condtac; try apply Time.bot_spec. subst. refl.
-          - unfold View.singleton_rw. econs; ss; try apply TimeMap.bot_spec.
-            ii. unfold TimeMap.singleton, LocFun.add, LocFun.find, LocFun.init.
-            condtac; try apply Time.bot_spec. subst. refl.
-        }
-        condtac; try apply View.join_bot_r.
-        apply View.le_join_l.
-        destruct released; eauto. apply View.bot_spec.
-      - rewrite (@View.le_join_l acq); cycle 1.
-        { etrans; [|eapply WF]. ss.
-          unfold View.singleton_ur_if. condtac; ss.
-          - unfold View.singleton_ur. econs; ss.
-            + ii. unfold TimeMap.singleton, LocFun.add, LocFun.find, LocFun.init.
-              condtac; try apply Time.bot_spec. subst.
-              rewrite CUR0; ss. refl.
-            + ii. unfold TimeMap.singleton, LocFun.add, LocFun.find, LocFun.init.
-              condtac; try apply Time.bot_spec. subst. refl.
-          - unfold View.singleton_rw. econs; ss; try apply TimeMap.bot_spec.
-            ii. unfold TimeMap.singleton, LocFun.add, LocFun.find, LocFun.init.
-            condtac; try apply Time.bot_spec. subst. refl.
-        }
-        condtac; try apply View.join_bot_r.
-        apply View.le_join_l.
-        etrans; [|eapply WF]. ss.
-        destruct released; eauto. apply View.bot_spec.
-    Qed.
-
-    Lemma stable_memory_tail
-          loc to rels mem
-          (STABLE: stable_memory ((loc, to) :: rels) mem):
-      stable_memory rels mem.
-    Proof.
-      ii. des.
-      - eapply STABLE; eauto.
-      - eapply STABLE; eauto. right. s. right. ss.
-    Qed.
-
-
-    (* step *)
 
     Lemma promise
-          rels tview1 promises1 mem1 loc from to msg promises2 mem2 kind
-          (TVIEW1: TView.closed tview1 mem1)
-          (MEM1: Memory.closed mem1)
-          (NORMAL_TVIEW1: normal_tview tview1)
+          promises1 mem1 loc from to msg promises2 mem2 kind
           (NORMAL_MEM1: normal_memory mem1)
-          (STABLE_TVIEW1: stable_tview mem1 tview1)
-          (STABLE_MEM1: stable_memory rels mem1)
           (MSG: forall val released
                   (MSG: msg = Message.concrete val (Some released)),
-              normal_view released /\ stable_view mem2 released)
+              normal_view released)
           (PROMISE: Memory.promise promises1 mem1 loc from to msg promises2 mem2 kind):
-      <<NORMAL_MEM2: normal_memory mem2>> /\
-      <<STABLE_TVIEW2: stable_tview mem2 tview1>> /\
-      <<STABLE_MEM2: stable_memory rels mem2>>.
+      <<NORMAL_MEM2: normal_memory mem2>>.
     Proof.
-      inv PROMISE; ss.
-      { (* add *)
-        splits.
-        - ii. revert GET.
-          erewrite Memory.add_o; eauto. condtac; ss; i.
-          + des. subst. inv GET.
-            exploit MSG; eauto. i. des. eauto.
-          + eapply NORMAL_MEM1; eauto.
-        - inv STABLE_TVIEW1. econs; ss; ii; revert GET.
-          + erewrite Memory.add_o; eauto. condtac; ss; i.
-            * des. subst. inv GET.
-              exploit Memory.add_get0; try exact MEM. i. des.
-              inv TVIEW1. specialize (REL0 loc0). inv REL0.
-              specialize (RLX loc). des. congr.
-            * eapply REL; eauto.
-          + erewrite Memory.add_o; eauto. condtac; ss; i; eauto.
-            des. subst. inv GET.
-            exploit Memory.add_get0; try exact MEM. i. des.
-            inv TVIEW1. inv CUR0.
-            specialize (RLX loc). des. congr.
-          + erewrite Memory.add_o; eauto. condtac; ss; i; eauto.
-            des. subst. inv GET.
-            exploit Memory.add_get0; try exact MEM. i. des.
-            inv TVIEW1. inv ACQ0.
-            specialize (RLX loc). des. congr.
-        - ii. revert GET.
-          erewrite Memory.add_o; eauto. condtac; ss; i.
-          + guardH LOC. des. subst. inv GET.
-            exploit MSG; eauto. i. des. eauto.
-          + guardH LOC. guardH o. inv MEM1. exploit CLOSED; eauto. i. des.
-            inv MSG_CLOSED. inv CLOSED0. inv CLOSED1.
-            specialize (RLX loc1). des.
-            exploit Memory.add_get1; try exact RLX; eauto. i.
-            rewrite x0 in *. inv GET0.
-            eapply STABLE_MEM1; eauto.
-      }
-
-      { (* split *)
-        des. subst.
-        splits; ss.
-        - ii. revert GET.
-          erewrite Memory.split_o; eauto. repeat condtac; ss; i.
-          + des. subst. inv GET.
-            exploit MSG; eauto. i. des. eauto.
-          + guardH o. des. subst. inv GET.
-            exploit Memory.split_get0; try exact MEM. i. des.
-            eapply NORMAL_MEM1; eauto.
-          + eapply NORMAL_MEM1; eauto.
-        - inv STABLE_TVIEW1. econs; ss; ii; revert GET.
-          + erewrite Memory.split_o; eauto. repeat condtac; ss; i.
-            * des. subst. inv GET.
-              exploit Memory.split_get0; try exact MEM. i. des.
-              inv TVIEW1. specialize (REL0 loc0). inv REL0.
-              specialize (RLX loc). des. congr.
-            * guardH o. des. subst. inv GET.
-              exploit Memory.split_get0; try exact MEM. i. des.
-              eapply REL; eauto.
-            * eapply REL; eauto.
-          + erewrite Memory.split_o; eauto. repeat condtac; ss; i; eauto.
-            * des. subst. inv GET.
-              exploit Memory.split_get0; try exact MEM. i. des.
-              inv TVIEW1. inv CUR0.
-              specialize (RLX loc). des. congr.
-            * guardH o. des. subst. inv GET.
-              exploit Memory.split_get0; try exact MEM. i. des. eauto.
-          + erewrite Memory.split_o; eauto. repeat condtac; ss; i; eauto.
-            * des. subst. inv GET.
-              exploit Memory.split_get0; try exact MEM. i. des.
-              inv TVIEW1. inv ACQ0.
-              specialize (RLX loc). des. congr.
-            * guardH o. des. subst. inv GET.
-              exploit Memory.split_get0; try exact MEM. i. des. eauto.
-        - ii. revert GET.
-          erewrite Memory.split_o; eauto. repeat condtac; ss; i.
-          + guardH LOC. des. subst. inv GET.
-            exploit MSG; eauto. i. des. eauto.
-          + guardH LOC. guardH o. des. subst. inv GET.
-            exploit Memory.split_get0; try exact MEM. i. des.
-            inv MEM1. exploit CLOSED; try exact GET1. i. des.
-            inv MSG_CLOSED. inv CLOSED0. inv CLOSED1.
-            specialize (RLX loc1). des.
-            exploit Memory.split_get1; try exact RLX; eauto. i. des.
-            rewrite GET4 in *. inv GET0.
-            eapply STABLE_MEM1; eauto.
-          + guardH LOC. guardH o. guardH o0.
-            inv MEM1. exploit CLOSED; eauto. i. des.
-            inv MSG_CLOSED. inv CLOSED0. inv CLOSED1.
-            specialize (RLX loc1). des.
-            exploit Memory.split_get1; try exact RLX; eauto. i. des.
-            rewrite GET2 in *. inv GET0.
-            eapply STABLE_MEM1; eauto.
-      }
-
-      { (* lower *)
-        splits; ss.
-        - ii. revert GET.
-          erewrite Memory.lower_o; eauto. condtac; ss; i.
-          + des. subst. inv GET.
-            exploit MSG; eauto. i. des. eauto.
-          + eapply NORMAL_MEM1; eauto.
-        - inv STABLE_TVIEW1. econs; ss; ii; revert GET.
-          + erewrite Memory.lower_o; eauto. condtac; ss; i.
-            * des. subst. inv GET.
-              exploit Memory.lower_get0; try exact MEM. i. des.
-              inv MSG_LE. inv RELEASED. etrans; eauto.
-              eapply REL; eauto.
-            * eapply REL; eauto.
-          + erewrite Memory.lower_o; eauto. condtac; ss; i; eauto.
-            des. subst. inv GET.
-            exploit Memory.lower_get0; try exact MEM. i. des.
-            inv MSG_LE. inv RELEASED. etrans; eauto.
-          + erewrite Memory.lower_o; eauto. condtac; ss; i; eauto.
-            des. subst. inv GET.
-            exploit Memory.lower_get0; try exact MEM. i. des.
-            inv MSG_LE. inv RELEASED. etrans; eauto.
-        - ii. revert GET.
-          erewrite Memory.lower_o; eauto. condtac; ss; i.
-          + guardH LOC. des. subst. inv GET.
-            exploit MSG; eauto. i. des. eauto.
-          + guardH LOC. guardH o. inv MEM1. exploit CLOSED; eauto. i. des.
-            inv MSG_CLOSED. inv CLOSED0. inv CLOSED1.
-            specialize (RLX loc1). des.
-            exploit Memory.lower_get1; try exact RLX; eauto. i. des.
-            rewrite GET2 in *. inv GET0. inv MSG_LE. inv RELEASED.
-            etrans; eauto.
-            eapply STABLE_MEM1; eauto.
-      }
-
-      { (* cancel *)
-        splits; ss.
-        - ii. revert GET.
-          erewrite Memory.remove_o; eauto. condtac; ss; i.
+      ii. revert GET. inv PROMISE; ss.
+      - erewrite Memory.add_o; eauto. condtac; ss; i.
+        + inv GET. eapply MSG; eauto.
+        + eapply NORMAL_MEM1; eauto.
+      - erewrite Memory.split_o; eauto. repeat condtac; ss; i.
+        + inv GET. eapply MSG; eauto.
+        + guardH o. des. inv GET.
+          exploit Memory.split_get0; try exact MEM. i. des.
           eapply NORMAL_MEM1; eauto.
-        - inv STABLE_TVIEW1. econs; ss; ii; revert GET.
-          + erewrite Memory.remove_o; eauto. condtac; ss; i.
-            eapply REL; eauto.
-          + erewrite Memory.remove_o; eauto. condtac; ss; i; eauto.
-          + erewrite Memory.remove_o; eauto. condtac; ss; i; eauto.
-        - ii. revert GET.
-          erewrite Memory.remove_o; eauto. condtac; ss; i.
-          guardH LOC. guardH o. inv MEM1. exploit CLOSED; eauto. i. des.
-          inv MSG_CLOSED. inv CLOSED0. inv CLOSED1.
-          specialize (RLX loc1). des.
-          exploit Memory.remove_get1; try exact RLX; eauto. i. des.
-          { subst. exploit Memory.remove_get0; try exact MEM. i. des. congr. }
-          rewrite GET2 in *. inv GET0.
-          eapply STABLE_MEM1; eauto.
-      }
+        + eapply NORMAL_MEM1; eauto.
+      - erewrite Memory.lower_o; eauto. condtac; ss; i.
+        + inv GET. eapply MSG; eauto.
+        + eapply NORMAL_MEM1; eauto.
+      - erewrite Memory.remove_o; eauto. condtac; ss; i.
+        eapply NORMAL_MEM1; eauto.
+    Qed.
+
+    Lemma write
+          promises1 mem1 loc from to msg promises2 mem2 kind
+          (NORMAL_MEM1: normal_memory mem1)
+          (MSG: forall val released
+                  (MSG: msg = Message.concrete val (Some released)),
+              normal_view released)
+          (WRITE: Memory.write promises1 mem1 loc from to msg promises2 mem2 kind):
+      <<NORMAL_MEM2: normal_memory mem2>>.
+    Proof.
+      inv WRITE. eauto using promise.
+    Qed.
+
+    Lemma write_na
+          ts promises1 mem1 loc from to msg promises2 mem2 msgs kinds kind
+          (NORMAL_MEM1: normal_memory mem1)
+          (WRITE: Memory.write_na ts promises1 mem1 loc from to msg promises2 mem2 msgs kinds kind):
+      <<NORMAL_MEM2: normal_memory mem2>>.
+    Proof.
+      induction WRITE.
+      - eapply write; eauto; ss.
+      - apply IHWRITE. eapply write; eauto.
+        unguard. des; subst; ss.
     Qed.
 
     Lemma promise_step
-          rels lc1 mem1 loc from to msg lc2 mem2 kind
-          (WF1: Local.wf lc1 mem1)
-          (MEM1: Memory.closed mem1)
-          (NORMAL_TVIEW1: normal_tview (Local.tview lc1))
+          lc1 mem1 loc from to msg lc2 mem2 kind
           (NORMAL_MEM1: normal_memory mem1)
-          (STABLE_TVIEW1: stable_tview mem1 (Local.tview lc1))
-          (STABLE_MEM1: stable_memory rels mem1)
-          (RELS_WF1: RelWrites.wf rels (Local.promises lc1) mem1)
           (MSG: forall val released
                   (MSG: msg = Message.concrete val (Some released)),
-              normal_view released /\ stable_view mem2 released)
+              normal_view released)
           (STEP: Local.promise_step lc1 mem1 loc from to msg lc2 mem2 kind):
-      <<NORMAL_TVIEW2: normal_tview (Local.tview lc2)>> /\
-      <<NORMAL_MEM2: normal_memory mem2>> /\
-      <<STABLE_TVIEW2: stable_tview mem2 (Local.tview lc2)>> /\
-      <<STABLE_MEM2: stable_memory rels mem2>> /\
-      <<RELS_WF2: RelWrites.wf rels (Local.promises lc2) mem2>>.
+      <<NORMAL_MEM2: normal_memory mem2>>.
     Proof.
-      inv STEP. exploit promise; try apply WF1; eauto. i. des.
-      splits; auto. ii. ss.
-      exploit RELS_WF1; eauto. i. des. split.
-      - inv PROMISE.
-        + erewrite Memory.add_o; eauto. condtac; ss.
-          des. subst. exploit Memory.add_get0; try exact MEM. i. des. congr.
-        + erewrite Memory.split_o; eauto. repeat condtac; ss.
-          * des. subst. exploit Memory.split_get0; try exact MEM. i. des. congr.
-          * guardH o. des. subst.
-            exploit Memory.split_get0; try exact PROMISES. i. des. congr.
-        + erewrite Memory.lower_o; eauto. condtac; ss.
-          des. subst. exploit Memory.lower_get0; try exact PROMISES. i. des. congr.
-        + erewrite Memory.remove_o; eauto. condtac; ss.
-      - destruct (Memory.op_kind_is_cancel kind) eqn:KIND.
-        + destruct kind; ss. inv PROMISE.
-          erewrite Memory.remove_o; eauto. condtac; ss; eauto.
-          des. subst. exploit Memory.remove_get0; try exact MEM. i. des. congr.
-        + exploit Memory.promise_get1; eauto. i. des. inv MSG_LE. eauto.
+      inv STEP. eapply promise; eauto.
     Qed.
 
-    Lemma read_step_loc_cur
-          rels lc1 mem1 loc to val released ord lc2
+    Lemma read_step
+          lc1 mem1 loc to val released ord lc2
           (WF1: Local.wf lc1 mem1)
-          (MEM1: Memory.closed mem1)
           (NORMAL_TVIEW1: normal_tview (Local.tview lc1))
           (NORMAL_MEM1: normal_memory mem1)
-          (STABLE_TVIEW1: stable_tview mem1 (Local.tview lc1))
-          (STABLE_MEM1: stable_memory rels mem1)
-          (LOC: L loc)
-          (TO: to = (TView.cur (Local.tview lc1)).(View.rlx) loc)
-          (STEP: Local.read_step lc1 mem1 loc to val released ord lc2):
-      <<LC2: lc2 = lc1>>.
+          (STEP: Local.read_step lc1 mem1 loc to val released ord lc2)
+          (TO: L loc -> Ordering.le ord Ordering.plain ->
+               to = (TView.cur (Local.tview lc1)).(View.rlx) loc):
+      <<NORMAL_TVIEW2: normal_tview (Local.tview lc2)>>.
     Proof.
-      unnw. inv STEP. destruct lc1. f_equal; ss.
-      unfold TView.read_tview. condtac; ss; [|condtac; [|destruct ord]; ss].
-      - condtac; [|destruct ord]; ss.
-        destruct tview; ss. f_equal; ss.
-        + repeat rewrite View.le_join_l; ss.
-          * eapply View.singleton_ur_spec; try apply WF1.
-            inv NORMAL_TVIEW1. rewrite CUR; ss. refl.
-          * destruct released; try apply View.bot_spec. ss.
-            inv STABLE_TVIEW1. eauto.
-          * eapply View.singleton_ur_spec; try apply WF1.
-            inv NORMAL_TVIEW1. rewrite CUR; ss. refl.
-        + repeat rewrite View.le_join_l; ss.
-          * inv WF1. ss. inv TVIEW_WF. ss. etrans; eauto.
-            eapply View.singleton_ur_spec; ss.
-            inv NORMAL_TVIEW1. rewrite CUR0; ss. refl.
-          * inv WF1. ss. inv TVIEW_WF. ss. etrans; eauto.
-            destruct released; try apply View.bot_spec. ss.
-            inv STABLE_TVIEW1. eauto.
-          * inv WF1. ss. inv TVIEW_WF. ss. etrans; eauto.
-            eapply View.singleton_ur_spec; ss.
-            inv NORMAL_TVIEW1. rewrite CUR0; ss. refl.
-      - destruct tview; ss. f_equal; ss.
-        + repeat rewrite View.le_join_l; ss.
-          * eapply View.singleton_ur_spec; try apply WF1.
-            inv NORMAL_TVIEW1. rewrite CUR; ss. refl.
-          * destruct released; try apply View.bot_spec.
-          * eapply View.singleton_ur_spec; try apply WF1.
-            inv NORMAL_TVIEW1. rewrite CUR; ss. refl.
-        + repeat rewrite View.le_join_l; ss.
-          * inv WF1. ss. inv TVIEW_WF. ss. etrans; eauto.
-            eapply View.singleton_ur_spec; ss.
-            inv NORMAL_TVIEW1. rewrite CUR0; ss. refl.
-          * inv WF1. ss. inv TVIEW_WF. ss. etrans; eauto.
-            destruct released; try apply View.bot_spec. ss.
-            inv STABLE_TVIEW1. eauto.
-          * inv WF1. ss. inv TVIEW_WF. ss. etrans; eauto.
-            eapply View.singleton_ur_spec; ss.
-            inv NORMAL_TVIEW1. rewrite CUR0; ss. refl.
-      - destruct tview; ss. f_equal; ss.
-        + repeat rewrite View.le_join_l; ss.
-          * eapply View.singleton_rw_spec; try apply WF1.
-            inv NORMAL_TVIEW1. rewrite CUR; ss. refl.
-          * destruct released; try apply View.bot_spec.
-          * eapply View.singleton_rw_spec; try apply WF1.
-            inv NORMAL_TVIEW1. rewrite CUR; ss. refl.
-        + repeat rewrite View.le_join_l; ss.
-          * inv WF1. ss. inv TVIEW_WF. ss. etrans; eauto.
-            eapply View.singleton_rw_spec; ss.
-            inv NORMAL_TVIEW1. rewrite CUR0; ss. refl.
-          * inv WF1. ss. inv TVIEW_WF. ss. etrans; eauto.
-            destruct released; try apply View.bot_spec.
-          * inv WF1. ss. inv TVIEW_WF. ss. etrans; eauto.
-            eapply View.singleton_rw_spec; ss.
-            inv NORMAL_TVIEW1. rewrite CUR0; ss. refl.
+      destruct lc1. inv NORMAL_TVIEW1. inv STEP. ss.
+      hexploit get_normal_view; eauto. i.
+      destruct (classic (L loc /\ Ordering.le ord Ordering.plain)).
+      { des. exploit TO; eauto. i. subst.
+        econs; ss.
+        - apply join_normal_view.
+          + rewrite View.le_join_l; ss.
+            apply View.singleton_ur_if_spec; try apply WF1.
+            condtac; try refl. rewrite CUR; ss. refl.
+          + condtac; ss.
+        - apply join_normal_view.
+          + rewrite View.le_join_l; ss.
+            apply View.singleton_ur_if_spec; try apply WF1.
+            condtac; try apply WF1. rewrite CUR; ss. apply WF1.
+          + condtac; ss.
+      }
+      { econs; ss.
+        - repeat apply join_normal_view; try condtac; ss.
+          unfold View.singleton_ur_if.
+          condtac; eauto using singleton_ur_normal_view.
+          destruct (L loc) eqn:LOC.
+          + exfalso. apply H0. destruct ord; ss.
+          + apply singleton_rw_normal_view; eauto. rewrite LOC. ss.
+        - condtac; repeat eapply join_normal_view; eauto; ss.
+          destruct (L loc) eqn:LOC.
+          + exfalso. apply H0. destruct ord; ss.
+          + apply singleton_rw_normal_view; eauto. rewrite LOC. ss.
+      }
     Qed.
 
-    Lemma read_step_loc_ra
-          rels lc1 mem1 loc to val released ord lc2
-          (WF1: Local.wf lc1 mem1)
-          (MEM1: Memory.closed mem1)
+    Lemma write_step
+          lc1 sc1 mem1 loc from to val releasedm released ord lc2 sc2 mem2 kind
           (NORMAL_TVIEW1: normal_tview (Local.tview lc1))
           (NORMAL_MEM1: normal_memory mem1)
-          (STABLE_TVIEW1: stable_tview mem1 (Local.tview lc1))
-          (STABLE_MEM1: stable_memory rels mem1)
-          (RELS_WF1: RelWrites.wf rels (Local.promises lc1) mem1)
-          (LOC: L loc)
-          (REL: List.In (loc, to) rels)
-          (ORD: Ordering.le Ordering.acqrel ord)
-          (STEP: Local.read_step lc1 mem1 loc to val released ord lc2):
-      <<NORMAL_TVIEW2: normal_tview (Local.tview lc2)>> /\
-      <<STABLE_TVIEW2: stable_tview mem1 (Local.tview lc2)>> /\
-      <<RELS_WF2: RelWrites.wf rels (Local.promises lc2) mem1>>.
-    Proof.
-      inv STEP. ss. splits; ss.
-      - inv NORMAL_TVIEW1. econs; ss.
-        + repeat eapply join_normal_view; ss.
-          { destruct ord; ss. }
-          { condtac; ss. destruct released; ss; eauto. }
-        + repeat eapply join_normal_view; ss.
-          { destruct ord; ss. }
-          { condtac; ss. destruct released; ss; eauto. }
-      - inv STABLE_TVIEW1. econs; ss.
-        + unfold View.singleton_ur_if.
-          repeat (condtac; [|destruct ord; ss]). ii.
-          destruct (Loc.eq_dec loc loc0); subst; ss.
-          * unfold TimeMap.join, View.singleton_ur_if,
-            TimeMap.singleton, LocFun.add, LocFun.init, LocFun.find in GET0.
-            revert GET0. condtac; ss. i.
-            rewrite TimeFacts.le_join_l in GET0; cycle 1.
-            { etrans; [|eapply Time.join_r].
-              inv MEM1. exploit CLOSED; try exact GET. i. des.
-              inv MSG_TS. ss. }
-            rewrite TimeFacts.le_join_r in GET0; cycle 1.
-            { inv READABLE. auto. }
-            rewrite GET0 in *. inv GET. ss.
-            etrans; [|apply View.join_r]. refl.
-          * unfold TimeMap.join, View.singleton_ur_if,
-            TimeMap.singleton, LocFun.add, LocFun.init, LocFun.find in GET0.
-            revert GET0. condtac; try congr; ss. i.
-            rewrite (@TimeFacts.le_join_l _ Time.bot) in GET0; try apply Time.bot_spec.
-            exploit Time.join_cases. i. des.
-            { rewrite x0 in GET0.
-              exploit CUR; eauto. i. etrans; eauto.
-              etrans; [|apply View.join_l].
-              etrans; [|apply View.join_l].
-              refl. }
-            { rewrite x0 in GET0. destruct released; ss; cycle 1.
-              { unfold TimeMap.bot in *.
-                inv MEM1. rewrite INHABITED in GET0. ss. }
-              exploit STABLE_MEM1; try exact GET; eauto. i.
-              etrans; eauto.
-              etrans; [|apply View.join_r].
-              refl. }
-        + unfold View.singleton_ur_if.
-          repeat (condtac; [|destruct ord; ss]). ii.
-          destruct (Loc.eq_dec loc loc0); subst; ss.
-          * unfold TimeMap.join, View.singleton_ur_if,
-            TimeMap.singleton, LocFun.add, LocFun.init, LocFun.find in GET0.
-            revert GET0. condtac; ss. i.
-            rewrite Time.join_assoc in GET0.
-            rewrite (@TimeFacts.le_join_l to) in GET0; cycle 1.
-            { inv MEM1. exploit CLOSED; try exact GET. i. des.
-              inv MSG_TS. ss. }
-            exploit Time.join_cases. i. des.
-            { rewrite x0 in GET0.
-              exploit ACQ; eauto. i. etrans; eauto.
-              etrans; [|apply View.join_l].
-              etrans; [|apply View.join_l].
-              refl. }
-            { rewrite x0 in GET0. rewrite GET0 in *. inv GET. ss.
-              etrans; [|apply View.join_r]. 
-              refl. }
-          * unfold TimeMap.join, View.singleton_ur_if,
-            TimeMap.singleton, LocFun.add, LocFun.init, LocFun.find in GET0.
-            revert GET0. condtac; try congr; ss. i.
-            rewrite (@TimeFacts.le_join_l _ Time.bot) in GET0; try apply Time.bot_spec.
-            exploit Time.join_cases. i. des.
-            { rewrite x0 in GET0.
-              exploit ACQ; eauto. i. etrans; eauto.
-              etrans; [|apply View.join_l].
-              etrans; [|apply View.join_l].
-              refl. }
-            { rewrite x0 in GET0. destruct released; ss; cycle 1.
-              { unfold TimeMap.bot in *.
-                inv MEM1. rewrite INHABITED in GET0. ss. }
-              exploit STABLE_MEM1; try exact GET; eauto. i.
-              etrans; eauto.
-              etrans; [|apply View.join_r].
-              refl. }
-    Qed.
-
-    Lemma read_step_other
-          rels lc1 mem1 loc to val released ord lc2
-          (WF1: Local.wf lc1 mem1)
-          (MEM1: Memory.closed mem1)
-          (NORMAL_TVIEW1: normal_tview (Local.tview lc1))
-          (NORMAL_MEM1: normal_memory mem1)
-          (STABLE_TVIEW1: stable_tview mem1 (Local.tview lc1))
-          (STABLE_MEM1: stable_memory rels mem1)
-          (RELS_WF1: RelWrites.wf rels (Local.promises lc1) mem1)
-          (LOC: ~ L loc)
-          (STEP: Local.read_step lc1 mem1 loc to val released ord lc2):
-      <<NORMAL_TVIEW2: normal_tview (Local.tview lc2)>> /\
-      <<STABLE_TVIEW2: stable_tview mem1 (Local.tview lc2)>> /\
-      <<RELS_WF2: RelWrites.wf rels (Local.promises lc2) mem1>>.
-    Proof.
-      inv STEP. ss. splits; ss.
-      - inv NORMAL_TVIEW1. econs; ss.
-        + repeat apply join_normal_view; ss.
-          * apply singleton_ur_if_normal_view. ss.
-          * condtac; ss. destruct released; ss. eauto.
-        + repeat apply join_normal_view; ss.
-          * apply singleton_ur_if_normal_view. ss.
-          * condtac; ss. destruct released; ss. eauto.
-      - inv STABLE_TVIEW1. econs; ss.
-        + repeat apply join_stable_view; ss.
-          * apply singleton_ur_if_stable_view; ss.
-          * condtac; ss.
-            { destruct released; ss.
-              - eapply STABLE_MEM1; eauto.
-              - apply bot_stable_view; ss. }
-            { apply bot_stable_view; ss. }
-        + repeat apply join_stable_view; ss.
-          * apply singleton_ur_if_stable_view; ss.
-          * condtac; ss.
-            { destruct released; ss.
-              - eapply STABLE_MEM1; eauto.
-              - apply bot_stable_view; ss. }
-            { apply bot_stable_view; ss. }
-    Qed.
-
-    Lemma write_step_loc
-          rels lc1 sc1 mem1 loc from to val releasedm released ord lc2 sc2 mem2 kind
-          (WF1: Local.wf lc1 mem1)
-          (SC1: Memory.closed_timemap sc1 mem1)
-          (MEM1: Memory.closed mem1)
-          (RELS_WF1: RelWrites.wf rels (Local.promises lc1) mem1)
-          (NORMAL_TVIEW1: normal_tview (Local.tview lc1))
-          (NORMAL_MEM1: normal_memory mem1)
-          (STABLE_TVIEW1: stable_tview mem1 (Local.tview lc1))
-          (STABLE_MEM1: stable_memory rels mem1)
-          (WF_RELEASEDM: View.opt_wf releasedm)
-          (CLOSED_RELEASEDM: Memory.closed_opt_view releasedm mem1)
-          (NORMAL_RELEASEDM: normal_view (View.unwrap releasedm))
-          (RELEASEDM: View.le (View.unwrap releasedm) (TView.cur (Local.tview lc1)))
-          (LOC: L loc)
+          (RELEASEDM: normal_view (View.unwrap releasedm))
           (STEP: Local.write_step lc1 sc1 mem1 loc from to val releasedm released ord lc2 sc2 mem2 kind):
-      <<NORMAL_TVIEW2: normal_tview (Local.tview lc2)>> /\
-      <<NORMAL_MEM2: normal_memory mem2>> /\
-      <<STABLE_TVIEW2: stable_tview mem2 (Local.tview lc2)>> /\
-      <<STABLE_MEM2: stable_memory (if Ordering.le Ordering.acqrel ord then (loc, to) :: rels else rels) mem2>> /\
-      <<RELS_WF2: RelWrites.wf (if Ordering.le Ordering.acqrel ord then (loc, to) :: rels else rels) 
-                                   (Local.promises lc2) mem2>>.
+      (<<NORMAL_TVIEW2: normal_tview (Local.tview lc2)>>) /\
+      (<<NORMAL_MEM2: normal_memory mem2>>).
     Proof.
-      exploit Local.write_step_future; eauto. i. des.
-      inv STEP. inv WRITE. ss.
-      assert (NORMAL_TVIEW2: normal_tview (TView.write_tview (Local.tview lc1) sc1 loc to ord)).
-      { inv NORMAL_TVIEW1.
-        econs; ss; i; try by (apply join_normal_view; ss).
-        unfold LocFun.add. condtac; eauto. subst.
-        condtac; apply join_normal_view; ss. }
-      assert (STABLE_TVIEW2: stable_tview mem2 (TView.write_tview (Local.tview lc1) sc1 loc to ord)).
-      { inv STABLE_TVIEW1. econs; ss; i.
-        - condtac; ss.
-          { unfold LocFun.add, LocFun.find.
-            condtac; ss; subst; ii; ss.
-            inv WF1. inv TVIEW_WF. inv TVIEW_CLOSED.
-            destruct (REL1 loc0). specialize (RLX loc1). des.
-            exploit Memory.promise_get1; try exact RLX; eauto.
-            { inv PROMISE; ss. }
-            i. des.
-            rewrite GET0 in *. inv GET. inv MSG_LE. inv RELEASED.
-            etrans; eauto. eapply REL; eauto.
-          }
-          { unfold LocFun.add, LocFun.find.
-            condtac; ss; subst; ii; ss.
-            inv WF1. inv TVIEW_WF. inv TVIEW_CLOSED.
-            destruct (REL1 loc0). specialize (RLX loc1). des.
-            exploit Memory.promise_get1; try exact RLX; eauto.
-            { inv PROMISE; ss. }
-            i. des.
-            rewrite GET0 in *. inv GET. inv MSG_LE. inv RELEASED.
-            etrans; eauto. eapply REL; eauto.
-          }
-        - ii. revert GET. ss.
-          unfold TimeMap.join, TimeMap.singleton, LocFun.add, LocFun.init, LocFun.find.
-          condtac; ss; subst; i.
-          + rewrite TimeFacts.le_join_r in GET; cycle 1.
-            { inv WRITABLE. econs. ss. }
-            exploit Memory.promise_get0; try exact PROMISE.
-            { inv PROMISE; ss. }
-            i. des.
-            rewrite GET in *. inv GET_MEM.
-            revert H2. unfold TView.write_released. condtac; ss.
-            unfold LocFun.add. repeat condtac; ss.
-            * i. inv H2.
-              repeat eapply View.join_spec; eauto using View.join_l, View.join_r.
-            * i. inv H2.
-              repeat eapply View.join_spec; eauto using View.join_l, View.join_r.
-              etrans; try eapply WF1. apply View.join_l.
-          + rewrite TimeFacts.le_join_l in GET; try by apply Time.bot_spec.
-            etrans; [|apply View.join_l].
-            revert GET. inv PROMISE.
-            { erewrite Memory.add_o; eauto. condtac; ss; i; eauto.
-              des. subst. inv GET. ss. }
-            { erewrite Memory.split_o; eauto. repeat condtac; ss; i; eauto.
-              - des. subst. inv GET. ss.
-              - guardH o. des. subst. inv GET. ss. }
-            { erewrite Memory.lower_o; eauto. condtac; ss; i; eauto.
-              des. subst. inv GET. ss. }
-            { exploit Memory.remove_get0; try exact PROMISES. i. des.
-              exploit Memory.remove_get0; try exact REMOVE. i. des.
-              congr. }
-        - ii.  revert GET. ss.
-          unfold TimeMap.join, TimeMap.singleton, LocFun.add, LocFun.init, LocFun.find.
-          condtac; ss; subst; i.
-          + exploit Time.join_cases. i. des.
-            * erewrite x0 in GET.
-              inv WF1. inv TVIEW_CLOSED. inv ACQ0.
-              destruct (RLX loc). des.
-              exploit Memory.promise_get1; try exact H; eauto.
-              { inv PROMISE; ss. }
-              i. des.
-              rewrite GET0 in *. inv GET. inv MSG_LE. inv RELEASED.
-              etrans; eauto.
-              etrans; [|apply View.join_l].
-              eauto.
-            * erewrite x0 in GET.
-              exploit Memory.promise_get0; try exact PROMISE.
-              { inv PROMISE; ss. }
-              i. des.
-              rewrite GET in *. inv GET_MEM.
-              revert H2. unfold TView.write_released. condtac; ss.
-              unfold LocFun.add. repeat condtac; ss.
-              { i. inv H2.
-                repeat eapply View.join_spec; try apply View.join_r.
-                - etrans; eauto.
-                  etrans; try eapply WF1. apply View.join_l.
-                - etrans; try eapply WF1. apply View.join_l. }
-              { i. inv H2.
-                repeat eapply View.join_spec; try apply View.join_r.
-                - etrans; eauto.
-                  etrans; try eapply WF1. apply View.join_l.
-                - etrans; try eapply WF1. etrans; try eapply WF1. apply View.join_l. }
-          + rewrite TimeFacts.le_join_l in GET; try by apply Time.bot_spec.
-            etrans; [|apply View.join_l].
-            revert GET. inv PROMISE.
-            { erewrite Memory.add_o; eauto. condtac; ss; i; eauto.
-              des. subst. inv GET. ss. }
-            { erewrite Memory.split_o; eauto. repeat condtac; ss; i; eauto.
-              - des. subst. inv GET. ss.
-              - guardH o. des. subst. inv GET. ss. }
-            { erewrite Memory.lower_o; eauto. condtac; ss; i; eauto.
-              des. subst. inv GET. ss. }
-            { exploit Memory.remove_get0; try exact PROMISES. i. des.
-              exploit Memory.remove_get0; try exact REMOVE. i. des.
-              congr. }
-      }
-
-      assert (NORMAL_RELEASED: forall released,
-                 TView.write_released (Local.tview lc1) sc1 loc to releasedm ord = Some released ->
-                 normal_view released).
-      { unfold TView.write_released. repeat (condtac; ss).
-        unfold LocFun.add. condtac; ss.
-        - i. inv H. repeat apply join_normal_view; ss. apply NORMAL_TVIEW1.
-        - i. inv H. unfold LocFun.add. condtac; ss.
-          repeat apply join_normal_view; ss. apply NORMAL_TVIEW1. }
-
-      condtac; ss.
-      { assert (RELEASED: TView.write_released (Local.tview lc1) sc1 loc to releasedm ord =
-                          Some (View.join (View.singleton_ur loc to) (TView.cur (Local.tview lc1)))).
-        { unfold TView.write_released. repeat (condtac; ss); cycle 1.
-          { destruct ord; ss. }
-          f_equal.
-          unfold LocFun.add. condtac; ss.
-          rewrite (View.join_comm (View.singleton_ur loc to)).
-          apply View.antisym; cycle 1.
-          { etrans; [|eapply View.join_r]. refl. }
-          apply View.join_spec; try refl.
-          etrans; [|eapply View.join_l]. ss.
-        }
-        assert (STABLE_RELEASED:
-                  stable_view mem2 (View.join (View.singleton_ur loc to) (TView.cur (Local.tview lc1)))).
-        { rewrite RELEASED in *. ii. revert GET. ss.
-          unfold TimeMap.join, TimeMap.singleton, LocFun.add, LocFun.init, LocFun.find. condtac; ss.
-          - subst. replace (Time.join to (View.rlx (TView.cur (Local.tview lc1)) loc)) with to; cycle 1.
-            { rewrite TimeFacts.le_join_l; ss.
-              inv WRITABLE. econs. ss. }
-            exploit Memory.promise_get0; try exact PROMISE; try by (inv PROMISE; ss). i. des.
-            rewrite GET_MEM in *. inv GET. refl.
-          - rewrite TimeFacts.le_join_r; try by apply Time.bot_spec. i.
-            inv WF1. inv TVIEW_CLOSED. inv CUR. specialize (RLX loc0). des.
-            exploit Memory.promise_get1; try exact RLX; eauto; try by (inv PROMISE; ss). i. des.
-            rewrite GET0 in *. inv GET. inv MSG_LE. inv RELEASED0.
-            etrans; eauto. etrans; [|apply View.join_r].
-            eapply STABLE_TVIEW1; eauto.
-        }
-        exploit promise; try exact PROMISE; try apply WF1; eauto.
-        { i. inv MSG. rewrite RELEASED in *. inv H1. split; ss.
-          apply join_normal_view.
-          eauto using singleton_ur_normal_view.
-          apply NORMAL_TVIEW1. }
-        i. des. splits; auto.
-        - ii. ss. des.
-          + eapply STABLE_MEM2; eauto.
-          + inv LOC0. exploit Memory.promise_get0; try exact PROMISE; try by (inv PROMISE; ss). i. des.
-            rewrite GET in *. inv GET_MEM.
-            rewrite RELEASED in *. inv H2.
-            eapply STABLE_RELEASED; eauto.
-          + eapply STABLE_MEM2; eauto.
-        - ii. ss. des.
-          + inv IN. exploit Memory.promise_get2; eauto; try by (inv PROMISE; ss). i. des.
-            exploit Memory.remove_get0; eauto. i. des. eauto.
-          + exploit RELS_WF1; eauto. i. des.
-            exploit Memory.promise_get1; try exact x0; eauto; try by (inv PROMISE; ss). i. des.
-            inv MSG_LE. esplits; eauto.
-            erewrite Memory.remove_o; eauto. condtac; ss.
-            guardH o. inv PROMISE; ss.
-            * erewrite Memory.add_o; eauto. condtac; ss.
-            * erewrite Memory.split_o; eauto. repeat condtac; ss.
-              guardH o0. des. subst.
-              exploit Memory.split_get0; try exact PROMISES. i. des. congr.
-            * erewrite Memory.lower_o; eauto. condtac; ss.
-      }
-
-      splits; auto.
-      - ii. revert GET. inv PROMISE; ss.
-        + erewrite Memory.add_o; eauto. condtac; ss.
-          * i. des. subst. inv GET.
-            eapply NORMAL_RELEASED; eauto.
-          * i. eapply NORMAL_MEM1; eauto.
-        + erewrite Memory.split_o; eauto. repeat condtac; ss.
-          * i. des. subst. inv GET.
-            eapply NORMAL_RELEASED; eauto.
-          * guardH o. des. subst. i. inv GET.
-            exploit Memory.split_get0; try exact MEM. i. des.
-            eapply NORMAL_MEM1; eauto.
-          * i. eapply NORMAL_MEM1; eauto.
-        + erewrite Memory.lower_o; eauto. condtac; ss.
-          * i. des. subst. inv GET.
-            eapply NORMAL_RELEASED; eauto.
-          * i. eapply NORMAL_MEM1; eauto.
-      - ii. guardH LOC0. revert GET. inv PROMISE; ss.
-        + erewrite Memory.add_o; eauto. condtac; ss.
-          * i. des. subst. inv GET. unguard. des; ss. subst.
-            exploit RELS_WF1; eauto. i. des.
-            exploit Memory.add_get0; try exact MEM. i. des. congr.
-          * guardH o. i. inv MEM1. exploit CLOSED; eauto. i. des.
-            inv MSG_CLOSED. inv CLOSED0. inv CLOSED1.
-            specialize (RLX loc1). des.
-            exploit Memory.add_get1; try exact RLX; eauto. i.
-            rewrite x0 in *. inv GET0. eapply STABLE_MEM1; eauto.
-        + erewrite Memory.split_o; eauto. repeat condtac; ss.
-          * i. des. subst. inv GET. unguard. des; ss.
-            exploit RELS_WF1; eauto. i. des.
-            exploit Memory.split_get0; try exact MEM. i. des. congr.
-          * guardH o. i. des. subst. inv GET.
-            exploit Memory.split_get0; try exact MEM. i. des.
-            inv MEM1. exploit CLOSED; try exact GET1. i. des.
-            inv MSG_CLOSED. inv CLOSED0. inv CLOSED1.
-            specialize (RLX loc1). des.
-            exploit Memory.split_get1; try exact RLX; eauto. i. des.
-            rewrite GET4 in *. inv GET0.
-            eapply STABLE_MEM1; eauto.
-          * guardH o. guardH o0. i.
-            inv MEM1. exploit CLOSED; eauto. i. des.
-            inv MSG_CLOSED. inv CLOSED0. inv CLOSED1.
-            specialize (RLX loc1). des.
-            exploit Memory.split_get1; try exact RLX; eauto. i. des.
-            rewrite GET2 in *. inv GET0. eapply STABLE_MEM1; eauto.
-        + erewrite Memory.lower_o; eauto. condtac; ss.
-          * i. des. subst. inv GET. unguard. des; ss.
-            exploit RELS_WF1; eauto. i. des.
-            exploit Memory.lower_get0; try exact PROMISES. i. des. congr.
-          * guardH o. i. inv MEM1. exploit CLOSED; eauto. i. des.
-            inv MSG_CLOSED. inv CLOSED0. inv CLOSED1.
-            specialize (RLX loc1). des.
-            exploit Memory.lower_get1; try exact RLX; eauto. i. des. inv MSG_LE.
-            rewrite GET2 in *. inv GET0. inv RELEASED.
-            etrans; eauto. eapply STABLE_MEM1; eauto.
-      - ii. ss. exploit RELS_WF1; eauto. i. des.
-        exploit Memory.promise_get1; try exact x0; eauto; try by (inv PROMISE; ss). i. des.
-        inv MSG_LE. esplits; eauto.
-        erewrite Memory.remove_o; eauto. condtac; ss. guardH o.
-        inv PROMISE; ss.
-        + erewrite Memory.add_o; eauto. condtac; ss.
-        + erewrite Memory.split_o; eauto. repeat condtac; ss.
-          guardH o0. des. subst.
-          exploit Memory.split_get0; try exact PROMISES. i. des. congr.
-        + erewrite Memory.lower_o; eauto. condtac; ss.
-    Qed.
-
-    Lemma write_step_loc_None
-          rels lc1 sc1 mem1 loc from to val released ord lc2 sc2 mem2 kind
-          (WF1: Local.wf lc1 mem1)
-          (SC1: Memory.closed_timemap sc1 mem1)
-          (MEM1: Memory.closed mem1)
-          (NORMAL_TVIEW1: normal_tview (Local.tview lc1))
-          (NORMAL_MEM1: normal_memory mem1)
-          (STABLE_TVIEW1: stable_tview mem1 (Local.tview lc1))
-          (STABLE_MEM1: stable_memory rels mem1)
-          (RELS_WF1: RelWrites.wf rels (Local.promises lc1) mem1)
-          (LOC: L loc)
-          (STEP: Local.write_step lc1 sc1 mem1 loc from to val None released ord lc2 sc2 mem2 kind):
-      <<NORMAL_TVIEW2: normal_tview (Local.tview lc2)>> /\
-      <<NORMAL_MEM2: normal_memory mem2>> /\
-      <<STABLE_TVIEW2: stable_tview mem2 (Local.tview lc2)>> /\
-      <<STABLE_MEM2: stable_memory (if Ordering.le Ordering.acqrel ord then (loc, to) :: rels else rels) mem2>> /\
-      <<RELS_WF2: RelWrites.wf (if Ordering.le Ordering.acqrel ord then (loc, to) :: rels else rels) 
-                                   (Local.promises lc2) mem2>>.
-    Proof.
-      eapply write_step_loc; eauto; ss.
-      - apply View.bot_spec.
-    Qed.
-
-    Lemma write_step_other
-          rels lc1 sc1 mem1 loc from to val releasedm released ord lc2 sc2 mem2 kind
-          (WF1: Local.wf lc1 mem1)
-          (SC1: Memory.closed_timemap sc1 mem1)
-          (MEM1: Memory.closed mem1)
-          (NORMAL_TVIEW1: normal_tview (Local.tview lc1))
-          (NORMAL_MEM1: normal_memory mem1)
-          (STABLE_TVIEW1: stable_tview mem1 (Local.tview lc1))
-          (STABLE_MEM1: stable_memory rels mem1)
-          (RELS_WF1: RelWrites.wf rels (Local.promises lc1) mem1)
-          (LOC: ~ L loc)
-          (WF_RELEASEDM: View.opt_wf releasedm)
-          (CLOSED_RELEASEDM: Memory.closed_opt_view releasedm mem1)
-          (NORMAL_RELEASEDM: normal_view (View.unwrap releasedm))
-          (STABLE_RELEASEDM: stable_view mem1 (View.unwrap releasedm))
-          (STEP: Local.write_step lc1 sc1 mem1 loc from to val releasedm released ord lc2 sc2 mem2 kind):
-      <<NORMAL_TVIEW2: normal_tview (Local.tview lc2)>> /\
-      <<NORMAL_MEM2: normal_memory mem2>> /\
-      <<STABLE_TVIEW2: stable_tview mem2 (Local.tview lc2)>> /\
-      <<STABLE_MEM2: stable_memory rels mem2>> /\
-      <<RELS_WF2: RelWrites.wf rels (Local.promises lc2) mem2>>.
-    Proof.
-      exploit Local.write_step_future; eauto. i. des.
-      inv STEP. inv WRITE. ss.
-      assert (NORMAL_TVIEW2: normal_tview (TView.write_tview (Local.tview lc1) sc1 loc to ord)).
-      { inv NORMAL_TVIEW1.
-        econs; ss; i; try by (apply join_normal_view; ss).
-        unfold LocFun.add. condtac; eauto. subst.
-        condtac; apply join_normal_view; ss. }
-      assert (STABLE_TVIEW2: stable_tview mem2 (TView.write_tview (Local.tview lc1) sc1 loc to ord)).
-      { inv STABLE_TVIEW1. econs; ss; i.
-        { condtac; ss.
-          - unfold LocFun.add, LocFun.find.
-            condtac; ss; subst; ii; ss.
-            + revert GET.
-              unfold TimeMap.join, TimeMap.singleton, LocFun.add, LocFun.init, LocFun.find.
-              condtac; ss; i.
-              * subst. congr.
-              * rewrite TimeFacts.le_join_l in GET; try by apply Time.bot_spec.
-                etrans; [|eapply View.join_l].
-                revert GET. inv PROMISE.
-                { erewrite Memory.add_o; eauto. condtac; ss; i; eauto.
-                  des. subst. inv GET. ss. }
-                { erewrite Memory.split_o; eauto. repeat condtac; ss; i; eauto.
-                  - des. subst. inv GET. ss.
-                  - guardH o. des. subst. inv GET. ss. }
-                { erewrite Memory.lower_o; eauto. condtac; ss; i; eauto.
-                  des. subst. inv GET. ss. }
-                { exploit Memory.remove_get0; try exact PROMISES. i. des.
-                  exploit Memory.remove_get0; try exact REMOVE. i. des.
-                  congr. }
-            + inv WF1. inv TVIEW_WF. inv TVIEW_CLOSED.
-              destruct (REL1 loc0). specialize (RLX loc1). des.
-              exploit Memory.promise_get1; try exact RLX; eauto.
-              { inv PROMISE; ss. }
-              i. des.
-              rewrite GET0 in *. inv GET. inv MSG_LE. inv RELEASED.
-              etrans; eauto. eapply REL; eauto.
-          - unfold LocFun.add, LocFun.find.
-            condtac; ss; subst; ii; ss.
-            + revert GET.
-              unfold TimeMap.join, TimeMap.singleton, LocFun.add, LocFun.init, LocFun.find.
-              condtac; ss; i.
-              * subst. congr.
-              * rewrite TimeFacts.le_join_l in GET; try by apply Time.bot_spec.
-                etrans; [|eapply View.join_l].
-                revert GET. inv PROMISE.
-                { erewrite Memory.add_o; eauto. condtac; ss; i.
-                  - des. subst. inv GET. ss.
-                  - eapply REL; eauto. }
-                { erewrite Memory.split_o; eauto. repeat condtac; ss; i; eauto.
-                  - des. subst. inv GET. ss.
-                  - guardH o. des. subst. inv GET. ss.
-                  - eapply REL; eauto. }
-                { erewrite Memory.lower_o; eauto. condtac; ss; i.
-                  - des. subst. inv GET. ss.
-                  - eapply REL; eauto. }
-                { exploit Memory.remove_get0; try exact PROMISES. i. des.
-                  exploit Memory.remove_get0; try exact REMOVE. i. des.
-                  congr. }
-            + inv WF1. inv TVIEW_WF. inv TVIEW_CLOSED.
-              destruct (REL1 loc0). specialize (RLX loc1). des.
-              exploit Memory.promise_get1; try exact RLX; eauto.
-              { inv PROMISE; ss. }
-              i. des.
-              rewrite GET0 in *. inv GET. inv MSG_LE. inv RELEASED.
-              etrans; eauto. eapply REL; eauto.
-        }
-        { ii. revert GET. ss.
-          unfold TimeMap.join, TimeMap.singleton, LocFun.add, LocFun.init, LocFun.find.
-          condtac; ss; subst; i; try congr.
-          rewrite TimeFacts.le_join_l in GET; try by apply Time.bot_spec.
-          etrans; [|apply View.join_l].
-          revert GET. inv PROMISE.
-          { erewrite Memory.add_o; eauto. condtac; ss; i; eauto.
-            des. subst. inv GET. ss. }
-          { erewrite Memory.split_o; eauto. repeat condtac; ss; i; eauto.
-            - des. subst. inv GET. ss.
-            - guardH o. des. subst. inv GET. ss. }
-          { erewrite Memory.lower_o; eauto. condtac; ss; i; eauto.
-            des. subst. inv GET. ss. }
-          { exploit Memory.remove_get0; try exact PROMISES. i. des.
-            exploit Memory.remove_get0; try exact REMOVE. i. des.
-            congr. }
-        }
-        { ii.  revert GET. ss.
-          unfold TimeMap.join, TimeMap.singleton, LocFun.add, LocFun.init, LocFun.find.
-          condtac; ss; subst; i; try congr.
-          rewrite TimeFacts.le_join_l in GET; try by apply Time.bot_spec.
-          etrans; [|apply View.join_l].
-          revert GET. inv PROMISE.
-          { erewrite Memory.add_o; eauto. condtac; ss; i; eauto.
-            des. subst. inv GET. ss. }
-          { erewrite Memory.split_o; eauto. repeat condtac; ss; i; eauto.
-            - des. subst. inv GET. ss.
-            - guardH o. des. subst. inv GET. ss. }
-          { erewrite Memory.lower_o; eauto. condtac; ss; i; eauto.
-            des. subst. inv GET. ss. }
-          { exploit Memory.remove_get0; try exact PROMISES. i. des.
-            exploit Memory.remove_get0; try exact REMOVE. i. des.
-            congr. }
-        }
-      }
-
-      exploit promise; try exact PROMISE; try apply WF1; eauto.
-      { unfold TView.write_released. repeat (condtac; ss).
+      destruct lc1. inv NORMAL_TVIEW1. inv STEP. ss.
+      hexploit write; eauto.
+      { i. revert MSG. unfold TView.write_released.
+        condtac; ss. i. inv MSG.
+        condtac; repeat apply join_normal_view; eauto.
         - unfold LocFun.add. condtac; ss.
-          i. inv MSG. split.
-          + repeat apply join_normal_view; ss. apply NORMAL_TVIEW1.
-          + ii. revert GET.
-            destruct (Loc.eq_dec loc loc0); subst; try congr.
-            ss. unfold TimeMap.join, TimeMap.singleton, LocFun.add, LocFun.init, LocFun.find.
-            condtac; ss; try congr.
-            rewrite (@TimeFacts.le_join_l _ Time.bot); try by apply Time.bot_spec. i.
-            rewrite <- View.join_assoc.
-            etrans; [|apply View.join_l].
-            eapply future_stable_view; try eapply GET; try eapply join_stable_view; eauto.
-            * eapply Memory.join_closed_view; ss.
-              { inv CLOSED_RELEASEDM; ss.
-                apply Memory.closed_view_bot. apply MEM1. }
-              { apply WF1. }
-            * apply STABLE_TVIEW1.
+          apply join_normal_view; ss.
         - unfold LocFun.add. condtac; ss.
-          i. inv MSG. split.
-          + repeat apply join_normal_view; ss. apply NORMAL_TVIEW1.
-          + ii. revert GET.
-            destruct (Loc.eq_dec loc loc0); subst; try congr.
-            ss. unfold TimeMap.join, TimeMap.singleton, LocFun.add, LocFun.init, LocFun.find.
-            condtac; ss; try congr.
-            rewrite (@TimeFacts.le_join_l _ Time.bot); try by apply Time.bot_spec. i.
-            rewrite <- View.join_assoc.
-            etrans; [|apply View.join_l].
-            eapply future_stable_view; try eapply GET; try eapply join_stable_view; eauto.
-            * eapply Memory.join_closed_view; ss.
-              { inv CLOSED_RELEASEDM; ss.
-                apply Memory.closed_view_bot. apply MEM1. }
-              { apply WF1. }
-            * apply STABLE_TVIEW1. ss.
+          apply join_normal_view; ss.
       }
-
-      i. des. splits; auto.
-      ii. exploit RELS_WF1; eauto. i. des.
-      exploit Memory.promise_get1; try exact x0; eauto; try by (inv PROMISE; ss). i. des. inv MSG_LE.
-      esplits; eauto. s.
-      erewrite Memory.remove_o; eauto. condtac; ss. guardH o.
-      inv PROMISE; ss.
-      - erewrite Memory.add_o; eauto. condtac; ss.
-      - erewrite Memory.split_o; eauto. repeat condtac; ss.
-        guardH o0. des. subst.
-        exploit Memory.split_get0; try exact PROMISES. i. des. congr.
-      - erewrite Memory.lower_o; eauto. condtac; ss.
+      i. des. splits; ss.
+      econs; repeat apply join_normal_view; ss;
+        try apply singleton_ur_normal_view. i.
+      unfold LocFun.add.
+      repeat condtac; ss; eauto;
+        repeat apply join_normal_view; ss.
     Qed.
 
-    Lemma write_step_other_None
-          rels lc1 sc1 mem1 loc from to val released ord lc2 sc2 mem2 kind
-          (WF1: Local.wf lc1 mem1)
-          (SC1: Memory.closed_timemap sc1 mem1)
-          (MEM1: Memory.closed mem1)
+    Lemma write_na_step
+          lc1 sc1 mem1 loc from to val ord lc2 sc2 mem2 msgs kinds kind
           (NORMAL_TVIEW1: normal_tview (Local.tview lc1))
           (NORMAL_MEM1: normal_memory mem1)
-          (STABLE_TVIEW1: stable_tview mem1 (Local.tview lc1))
-          (STABLE_MEM1: stable_memory rels mem1)
-          (RELS_WF1: RelWrites.wf rels (Local.promises lc1) mem1)
-          (LOC: ~ L loc)
-          (STEP: Local.write_step lc1 sc1 mem1 loc from to val None released ord lc2 sc2 mem2 kind):
-      <<NORMAL_TVIEW2: normal_tview (Local.tview lc2)>> /\
-      <<NORMAL_MEM2: normal_memory mem2>> /\
-      <<STABLE_TVIEW2: stable_tview mem2 (Local.tview lc2)>> /\
-      <<STABLE_MEM2: stable_memory rels mem2>> /\
-      <<RELS_WF2: RelWrites.wf rels (Local.promises lc2) mem2>>.
+          (STEP: Local.write_na_step lc1 sc1 mem1 loc from to val ord lc2 sc2 mem2 msgs kinds kind):
+      (<<NORMAL_TVIEW2: normal_tview (Local.tview lc2)>>) /\
+      (<<NORMAL_MEM2: normal_memory mem2>>).
     Proof.
-      eapply write_step_other; eauto; ss.
-      apply bot_stable_view. apply MEM1.
+      destruct lc1. inv NORMAL_TVIEW1. inv STEP. ss.
+      hexploit write_na; eauto. i. des. splits; ss.
+      econs; repeat apply join_normal_view; ss;
+        try apply singleton_ur_normal_view. i.
+      unfold LocFun.add.
+      repeat condtac; ss; eauto;
+        repeat apply join_normal_view; ss.
     Qed.
 
     Lemma fence_step
-          rels lc1 sc1 mem1 ordr ordw lc2 sc2
+          lc1 sc1 ordr ordw lc2 sc2
+          (NORMAL_TVIEW1: normal_tview (Local.tview lc1))
+          (STEP: Local.fence_step lc1 sc1 ordr ordw lc2 sc2):
+      (<<NORMAL_TVIEW2: normal_tview (Local.tview lc2)>>).
+    Proof.
+      inv NORMAL_TVIEW1. inv STEP. ss.
+      econs; ss; i; repeat condtac; ss;
+        repeat apply join_normal_view; ss.
+    Qed.
+
+    Lemma ord_program_step
+          ordcr ordcw e lc1 sc1 mem1 lc2 sc2 mem2
           (WF1: Local.wf lc1 mem1)
           (NORMAL_TVIEW1: normal_tview (Local.tview lc1))
-          (STABLE_TVIEW1: stable_tview mem1 (Local.tview lc1))
-          (STABLE_SC1: stable_timemap mem1 sc1)
-          (RELS_WF1: RelWrites.wf rels (Local.promises lc1) mem1)
-          (STEP: Local.fence_step lc1 sc1 ordr ordw lc2 sc2):
-      <<NORMAL_TVIEW2: normal_tview (Local.tview lc2)>> /\
-      <<STABLE_TVIEW2: stable_tview mem1 (Local.tview lc2)>> /\
-      <<STABLE_SC2: stable_timemap mem1 sc2>> /\
-      <<RELS_WF2: RelWrites.wf rels (Local.promises lc2) mem1>>.
+          (NORMAL_MEM1: normal_memory mem1)
+          (STEP: OrdLocal.program_step L ordcr ordcw e lc1 sc1 mem1 lc2 sc2 mem2)
+          (READ: forall loc to val released ord
+                   (EVENT: ThreadEvent.is_reading e = Some (loc, to, val, released, ord))
+                   (LOC: L loc)
+                   (ORD: Ordering.le ord Ordering.plain),
+              to = (TView.cur (Local.tview lc1)).(View.rlx) loc):
+      (<<NORMAL_TVIEW2: normal_tview (Local.tview lc2)>>) /\
+      (<<NORMAL_MEM2: normal_memory mem2>>).
     Proof.
-      inv STEP. ss. splits; ss.
-      - inv NORMAL_TVIEW1.
-        econs; ss; i; repeat (condtac; ss).
-        + apply join_normal_view; ss.
-        + apply join_normal_view; ss.
-      - inv STABLE_TVIEW1.
-        econs; ss; i; repeat (condtac; ss); eauto.
-        + unfold TView.write_fence_sc. repeat (condtac; ss).
-          * hexploit join_stable_view; [apply STABLE_SC1| apply ACQ|]. i.
-            unfold View.join in H. ss. ii.
-            etrans; [eapply H; eauto|].
-            econs; try refl. ss.
-            apply TimeMap.join_spec.
-            { apply TimeMap.join_l. }
-            { etrans; [|apply TimeMap.join_r]. apply WF1. }
-          * hexploit join_stable_view; [apply STABLE_SC1| apply CUR|]. i.
-            unfold View.join in H. ss. ii.
-            etrans; [eapply H; eauto|].
-            econs; try refl. ss.
-            apply TimeMap.join_spec.
-            { apply TimeMap.join_l. }
-            { etrans; [|apply TimeMap.join_r]. apply WF1. }
-        + unfold TView.write_fence_sc. repeat (condtac; ss).
-          * hexploit join_stable_view; [apply STABLE_SC1| apply ACQ|]. i.
-            unfold View.join in H. ss. ii.
-            etrans; [eapply H; eauto|].
-            econs; try refl. ss.
-            apply TimeMap.join_spec.
-            { apply TimeMap.join_l. }
-            { etrans; [|apply TimeMap.join_r]. apply WF1. }
-          * hexploit join_stable_view; [apply STABLE_SC1| apply CUR|]. i.
-            unfold View.join in H. ss. ii.
-            etrans; [eapply H; eauto|].
-            econs; try refl. ss.
-            apply TimeMap.join_spec.
-            { apply TimeMap.join_l. }
-            { etrans; [|apply TimeMap.join_r]. apply WF1. }
-        + unfold TView.write_fence_sc. repeat (condtac; ss).
-          * apply join_stable_view; ss.
-            hexploit join_stable_view; [apply STABLE_SC1| apply ACQ|]. i.
-            unfold View.join in H. ss. ii.
-            etrans; [eapply H; eauto|].
-            econs; try refl. ss.
-            apply TimeMap.join_spec.
-            { apply TimeMap.join_l. }
-            { etrans; [|apply TimeMap.join_r]. apply WF1. }
-          * apply join_stable_view; ss.
-            hexploit join_stable_view; [apply STABLE_SC1| apply CUR|]. i.
-            unfold View.join in H. ss. ii.
-            etrans; [eapply H; eauto|].
-            econs; try refl. ss.
-            apply TimeMap.join_spec.
-            { apply TimeMap.join_l. }
-            { etrans; [|apply TimeMap.join_r]. apply WF1. }
-        + rewrite View.le_join_l; try by apply View.bot_spec. ss.
-      - unfold TView.write_fence_sc. repeat (condtac; ss).
-        + eapply join_stable_timemap; ss.
-          apply stable_view_stable_timemap.
-          * apply WF1.
-          * apply STABLE_TVIEW1.
-        + eapply join_stable_timemap; ss.
-          apply stable_view_stable_timemap.
-          * apply WF1.
-          * apply STABLE_TVIEW1.
+      inv STEP; ss.
+      - inv LOCAL. hexploit read_step; eauto.
+        i. exploit READ; eauto.
+        revert H0. condtac; ss. destruct ord, ordcr; ss.
+      - inv LOCAL. hexploit write_step; eauto. ss.
+      - inv LOCAL1. inv LOCAL2.
+        hexploit read_step; eauto.
+        { i. exploit READ; eauto.
+          revert H0. condtac; ss. destruct ordr, ordcr; ss.
+        }
+        i. des.
+        hexploit write_step; eauto.
+        inv STEP. ss. eapply get_normal_view; eauto.
+      - hexploit fence_step; eauto.
+      - hexploit fence_step; eauto.
+      - inv LOCAL. hexploit write_na_step; eauto.
     Qed.
+  End Normal.
+End Normal.
 
 
-    (* cap *)
+(* Module Stable. *)
+(*   Section Stable. *)
+(*     Variable L: Loc.t -> bool. *)
 
-    Lemma max_concrete_timemap_stable
-          mem tm
-          (CLOSED: Memory.closed mem)
-          (MAX: Memory.max_concrete_timemap mem tm):
-      stable_timemap mem tm.
-    Proof.
-      ii. dup CLOSED. inv CLOSED.
-      exploit CLOSED1; eauto. i. des. inv MSG_CLOSED. inv CLOSED. inv CLOSED2.
-      hexploit Memory.max_concrete_timemap_spec; try exact PLN; eauto. i.
-      hexploit Memory.max_concrete_timemap_spec; try exact RLX; eauto. i.
-      econs; ss.
-    Qed.
+(*     (* normal *) *)
 
-    Lemma cap_normal_memory
-          mem1 mem2
-          (CLOSED: Memory.closed mem1)
-          (CAP: Memory.cap mem1 mem2)
-          (NORMAL: normal_memory mem1):
-      normal_memory mem2.
-    Proof.
-      ii. exploit Memory.cap_inv; eauto. i. des; ss.
-      eapply NORMAL; eauto.
-    Qed.
+(*     Definition normal_view (view: View.t): Prop := *)
+(*       forall loc (LOC: L loc), (View.rlx view) loc = (View.pln view) loc. *)
 
-    Lemma cap_stable_view
-          mem1 mem2 view
-          (CLOSED: Memory.closed mem1)
-          (CAP: Memory.cap mem1 mem2)
-          (STABLE: stable_view mem1 view):
-      stable_view mem2 view.
-    Proof.
-      ii. exploit Memory.cap_inv; eauto. i. des; ss.
-      eapply STABLE; eauto.
-    Qed.
+(*     Inductive normal_tview (tview:TView.t): Prop := *)
+(*     | normal_tview_intro *)
+(*         (REL: forall loc, normal_view ((TView.rel tview) loc)) *)
+(*         (CUR: normal_view (TView.cur tview)) *)
+(*         (ACQ: normal_view (TView.acq tview)) *)
+(*     . *)
 
-    Lemma cap_stable_timemap
-          mem1 mem2 tm
-          (CLOSED: Memory.closed mem1)
-          (CAP: Memory.cap mem1 mem2)
-          (STABLE: stable_timemap mem1 tm):
-      stable_timemap mem2 tm.
-    Proof.
-      eapply cap_stable_view; eauto.
-    Qed.
+(*     Definition normal_memory (mem: Memory.t): Prop := *)
+(*       forall loc from to val released *)
+(*         (GET: Memory.get loc to mem = Some (from, Message.concrete val (Some released))), *)
+(*         normal_view released. *)
 
-    Lemma cap_stable_tview
-          mem1 mem2 tview
-          (CLOSED: Memory.closed mem1)
-          (CAP: Memory.cap mem1 mem2)
-          (STABLE: stable_tview mem1 tview):
-      stable_tview mem2 tview.
-    Proof.
-      inv STABLE. econs; eauto using cap_stable_view.
-    Qed.
+(*     Lemma join_normal_view *)
+(*           view1 view2 *)
+(*           (NORMAL1: normal_view view1) *)
+(*           (NORMAL2: normal_view view2): *)
+(*       normal_view (View.join view1 view2). *)
+(*     Proof. *)
+(*       ii. unfold normal_view in *. *)
+(*       destruct view1, view2. ss. *)
+(*       unfold TimeMap.join. *)
+(*       rewrite NORMAL1, NORMAL2; ss. *)
+(*     Qed. *)
 
-    Lemma cap_stable_memory
-          rels mem1 mem2
-          (CLOSED: Memory.closed mem1)
-          (CAP: Memory.cap mem1 mem2)
-          (STABLE: stable_memory rels mem1):
-      stable_memory rels mem2.
-    Proof.
-      ii. guardH LOC.
-      exploit Memory.cap_inv; try exact GET; eauto. i. des; ss.
-      exploit Memory.cap_inv; try exact GET0; eauto. i. des; ss.
-      eapply STABLE; eauto.
-    Qed.
-  End Stable.
-End Stable.
+(*     Lemma singleton_ur_normal_view loc ts: *)
+(*       normal_view (View.singleton_ur loc ts). *)
+(*     Proof. ss. Qed. *)
+
+(*     Lemma singleton_rw_normal_view *)
+(*           loc ts *)
+(*           (LOC: ~ L loc): *)
+(*       normal_view (View.singleton_rw loc ts). *)
+(*     Proof. *)
+(*       ii. ss. *)
+(*       unfold TimeMap.singleton, LocFun.add, LocFun.init, LocFun.find. *)
+(*       condtac; ss. subst. ss. *)
+(*     Qed. *)
+
+(*     Lemma singleton_ur_if_normal_view *)
+(*           b loc ts *)
+(*           (LOC: ~ L loc): *)
+(*       normal_view (View.singleton_ur_if b loc ts). *)
+(*     Proof. *)
+(*       unfold View.singleton_ur_if. condtac. *)
+(*       - apply singleton_ur_normal_view. *)
+(*       - apply singleton_rw_normal_view. ss. *)
+(*     Qed. *)
+
+
+(*     (* stable *) *)
+
+(*     Definition stable_view (mem: Memory.t) (view: View.t): Prop := *)
+(*       forall loc from val released *)
+(*         (LOC: L loc) *)
+(*         (GET: Memory.get loc ((View.rlx view) loc) mem = *)
+(*               Some (from, Message.concrete val (Some released))), *)
+(*         View.le released view. *)
+
+(*     Definition stable_timemap (mem: Memory.t) (tm: TimeMap.t): Prop := *)
+(*       stable_view mem (View.mk tm tm). *)
+
+(*     Inductive stable_tview (mem: Memory.t) (tview: TView.t): Prop := *)
+(*     | stable_tview_intro *)
+(*         (REL: forall loc (LOC: ~ L loc), stable_view mem ((TView.rel tview) loc)) *)
+(*         (CUR: stable_view mem (TView.cur tview)) *)
+(*         (ACQ: stable_view mem (TView.acq tview)) *)
+(*     . *)
+
+(*     Definition stable_memory (rels: Writes.t) (mem: Memory.t): Prop := *)
+(*       forall loc from to val released *)
+(*         (LOC: ~ L loc \/ List.In (loc, to) rels) *)
+(*         (GET: Memory.get loc to mem = Some (from, Message.concrete val (Some released))), *)
+(*         stable_view mem released. *)
+
+
+(*     Lemma future_stable_view *)
+(*           mem1 mem2 view *)
+(*           (CLOSED: Memory.closed_view view mem1) *)
+(*           (STABLE: stable_view mem1 view) *)
+(*           (MEM_FUTURE: Memory.future mem1 mem2): *)
+(*       stable_view mem2 view. *)
+(*     Proof. *)
+(*       ii. inv CLOSED. specialize (RLX loc). des. *)
+(*       exploit Memory.future_get1; try exact RLX; eauto. i. des. *)
+(*       rewrite GET0 in *. inv GET. inv MSG_LE. inv RELEASED. *)
+(*       exploit STABLE; eauto. *)
+(*     Qed. *)
+
+(*     Lemma future_stable_tview *)
+(*           mem1 mem2 tview *)
+(*           (CLOSED: TView.closed tview mem1) *)
+(*           (STABLE: stable_tview mem1 tview) *)
+(*           (MEM_FUTURE: Memory.future mem1 mem2): *)
+(*       stable_tview mem2 tview. *)
+(*     Proof. *)
+(*       destruct tview. inv CLOSED. inv STABLE. ss. *)
+(*       econs; ss; eauto using future_stable_view. *)
+(*     Qed. *)
+
+(*     Lemma join_stable_view *)
+(*           mem view1 view2 *)
+(*           (STABLE1: stable_view mem view1) *)
+(*           (STABLE2: stable_view mem view2): *)
+(*       stable_view mem (View.join view1 view2). *)
+(*     Proof. *)
+(*       ii. unfold stable_view in *. *)
+(*       unfold View.join, TimeMap.join in GET. ss. *)
+(*       exploit Time.join_cases. i. des. *)
+(*       - erewrite x0 in GET. *)
+(*         exploit STABLE1; eauto. i. *)
+(*         etrans; eauto. apply View.join_l. *)
+(*       - erewrite x0 in GET. *)
+(*         exploit STABLE2; eauto. i. *)
+(*         etrans; eauto. apply View.join_r. *)
+(*     Qed. *)
+
+(*     Lemma bot_stable_view *)
+(*           mem *)
+(*           (MEM: Memory.closed mem): *)
+(*       stable_view mem View.bot. *)
+(*     Proof. *)
+(*       ii. inv MEM. rewrite INHABITED in *. inv GET. *)
+(*     Qed. *)
+
+(*     Lemma singleton_ur_stable_view *)
+(*           mem loc ts *)
+(*           (MEM: Memory.closed mem) *)
+(*           (LOC: ~ L loc): *)
+(*       stable_view mem (View.singleton_ur loc ts). *)
+(*     Proof. *)
+(*       ii. revert GET. ss. *)
+(*       unfold TimeMap.singleton, LocFun.add, LocFun.init, LocFun.find. *)
+(*       condtac; subst; ss. i. *)
+(*       inv MEM. rewrite INHABITED in *. inv GET. *)
+(*     Qed. *)
+
+(*     Lemma singleton_rw_stable_view *)
+(*           mem loc ts *)
+(*           (MEM: Memory.closed mem) *)
+(*           (LOC: ~ L loc): *)
+(*       stable_view mem (View.singleton_rw loc ts). *)
+(*     Proof. *)
+(*       ii. revert GET. ss. *)
+(*       unfold TimeMap.singleton, LocFun.add, LocFun.init, LocFun.find. *)
+(*       condtac; subst; ss. i. *)
+(*       inv MEM. rewrite INHABITED in *. inv GET. *)
+(*     Qed. *)
+
+(*     Lemma singleton_ur_if_stable_view *)
+(*           mem b loc ts *)
+(*           (MEM: Memory.closed mem) *)
+(*           (LOC: ~ L loc): *)
+(*       stable_view mem (View.singleton_ur_if b loc ts). *)
+(*     Proof. *)
+(*       unfold View.singleton_ur_if. condtac. *)
+(*       - apply singleton_ur_stable_view; ss. *)
+(*       - apply singleton_rw_stable_view; ss. *)
+(*     Qed. *)
+
+(*     Lemma stable_view_stable_timemap *)
+(*           mem view *)
+(*           (VIEW: View.wf view) *)
+(*           (STABLE: stable_view mem view): *)
+(*       stable_timemap mem (View.rlx view). *)
+(*     Proof. *)
+(*       ii. etrans; [eapply STABLE|]; eauto. *)
+(*       econs; ss; try refl. apply VIEW. *)
+(*     Qed. *)
+
+(*     Lemma join_stable_timemap *)
+(*           mem tm1 tm2 *)
+(*           (STABLE1: stable_timemap mem tm1) *)
+(*           (STABLE2: stable_timemap mem tm2): *)
+(*       stable_timemap mem (TimeMap.join tm1 tm2). *)
+(*     Proof. *)
+(*       unfold stable_timemap in *. *)
+(*       hexploit join_stable_view; [exact STABLE1|exact STABLE2|]. ss. *)
+(*     Qed. *)
+
+(*     Lemma stable_tview_read_tview *)
+(*           mem tview *)
+(*           loc from val released ord *)
+(*           (WF: TView.wf tview) *)
+(*           (NORMAL: normal_tview tview) *)
+(*           (STABLE: stable_tview mem tview) *)
+(*           (LOC: L loc) *)
+(*           (GET: Memory.get loc ((View.rlx (TView.cur tview)) loc) mem = *)
+(*                 Some (from, Message.concrete val released)): *)
+(*       TView.read_tview tview loc ((View.rlx (TView.cur tview)) loc) released ord = tview. *)
+(*     Proof. *)
+(*       inv STABLE. inv NORMAL. *)
+(*       destruct tview. unfold TView.read_tview. ss. f_equal. *)
+(*       - rewrite (@View.le_join_l cur); cycle 1. *)
+(*         { unfold View.singleton_ur_if. condtac; ss. *)
+(*           - unfold View.singleton_ur. econs; ss. *)
+(*             + ii. unfold TimeMap.singleton, LocFun.add, LocFun.find, LocFun.init. *)
+(*               condtac; try apply Time.bot_spec. subst. *)
+(*               rewrite CUR0; ss. refl. *)
+(*             + ii. unfold TimeMap.singleton, LocFun.add, LocFun.find, LocFun.init. *)
+(*               condtac; try apply Time.bot_spec. subst. refl. *)
+(*           - unfold View.singleton_rw. econs; ss; try apply TimeMap.bot_spec. *)
+(*             ii. unfold TimeMap.singleton, LocFun.add, LocFun.find, LocFun.init. *)
+(*             condtac; try apply Time.bot_spec. subst. refl. *)
+(*         } *)
+(*         condtac; try apply View.join_bot_r. *)
+(*         apply View.le_join_l. *)
+(*         destruct released; eauto. apply View.bot_spec. *)
+(*       - rewrite (@View.le_join_l acq); cycle 1. *)
+(*         { etrans; [|eapply WF]. ss. *)
+(*           unfold View.singleton_ur_if. condtac; ss. *)
+(*           - unfold View.singleton_ur. econs; ss. *)
+(*             + ii. unfold TimeMap.singleton, LocFun.add, LocFun.find, LocFun.init. *)
+(*               condtac; try apply Time.bot_spec. subst. *)
+(*               rewrite CUR0; ss. refl. *)
+(*             + ii. unfold TimeMap.singleton, LocFun.add, LocFun.find, LocFun.init. *)
+(*               condtac; try apply Time.bot_spec. subst. refl. *)
+(*           - unfold View.singleton_rw. econs; ss; try apply TimeMap.bot_spec. *)
+(*             ii. unfold TimeMap.singleton, LocFun.add, LocFun.find, LocFun.init. *)
+(*             condtac; try apply Time.bot_spec. subst. refl. *)
+(*         } *)
+(*         condtac; try apply View.join_bot_r. *)
+(*         apply View.le_join_l. *)
+(*         etrans; [|eapply WF]. ss. *)
+(*         destruct released; eauto. apply View.bot_spec. *)
+(*     Qed. *)
+
+(*     Lemma stable_memory_tail *)
+(*           loc to rels mem *)
+(*           (STABLE: stable_memory ((loc, to) :: rels) mem): *)
+(*       stable_memory rels mem. *)
+(*     Proof. *)
+(*       ii. des. *)
+(*       - eapply STABLE; eauto. *)
+(*       - eapply STABLE; eauto. right. s. right. ss. *)
+(*     Qed. *)
+
+
+(*     (* step *) *)
+
+(*     Lemma promise *)
+(*           rels tview1 promises1 mem1 loc from to msg promises2 mem2 kind *)
+(*           (TVIEW1: TView.closed tview1 mem1) *)
+(*           (MEM1: Memory.closed mem1) *)
+(*           (NORMAL_TVIEW1: normal_tview tview1) *)
+(*           (NORMAL_MEM1: normal_memory mem1) *)
+(*           (STABLE_TVIEW1: stable_tview mem1 tview1) *)
+(*           (STABLE_MEM1: stable_memory rels mem1) *)
+(*           (MSG: forall val released *)
+(*                   (MSG: msg = Message.concrete val (Some released)), *)
+(*               normal_view released /\ stable_view mem2 released) *)
+(*           (PROMISE: Memory.promise promises1 mem1 loc from to msg promises2 mem2 kind): *)
+(*       <<NORMAL_MEM2: normal_memory mem2>> /\ *)
+(*       <<STABLE_TVIEW2: stable_tview mem2 tview1>> /\ *)
+(*       <<STABLE_MEM2: stable_memory rels mem2>>. *)
+(*     Proof. *)
+(*       inv PROMISE; ss. *)
+(*       { (* add *) *)
+(*         splits. *)
+(*         - ii. revert GET. *)
+(*           erewrite Memory.add_o; eauto. condtac; ss; i. *)
+(*           + des. subst. inv GET. *)
+(*             exploit MSG; eauto. i. des. eauto. *)
+(*           + eapply NORMAL_MEM1; eauto. *)
+(*         - inv STABLE_TVIEW1. econs; ss; ii; revert GET. *)
+(*           + erewrite Memory.add_o; eauto. condtac; ss; i. *)
+(*             * des. subst. inv GET. *)
+(*               exploit Memory.add_get0; try exact MEM. i. des. *)
+(*               inv TVIEW1. specialize (REL0 loc0). inv REL0. *)
+(*               specialize (RLX loc). des. congr. *)
+(*             * eapply REL; eauto. *)
+(*           + erewrite Memory.add_o; eauto. condtac; ss; i; eauto. *)
+(*             des. subst. inv GET. *)
+(*             exploit Memory.add_get0; try exact MEM. i. des. *)
+(*             inv TVIEW1. inv CUR0. *)
+(*             specialize (RLX loc). des. congr. *)
+(*           + erewrite Memory.add_o; eauto. condtac; ss; i; eauto. *)
+(*             des. subst. inv GET. *)
+(*             exploit Memory.add_get0; try exact MEM. i. des. *)
+(*             inv TVIEW1. inv ACQ0. *)
+(*             specialize (RLX loc). des. congr. *)
+(*         - ii. revert GET. *)
+(*           erewrite Memory.add_o; eauto. condtac; ss; i. *)
+(*           + guardH LOC. des. subst. inv GET. *)
+(*             exploit MSG; eauto. i. des. eauto. *)
+(*           + guardH LOC. guardH o. inv MEM1. exploit CLOSED; eauto. i. des. *)
+(*             inv MSG_CLOSED. inv CLOSED0. inv CLOSED1. *)
+(*             specialize (RLX loc1). des. *)
+(*             exploit Memory.add_get1; try exact RLX; eauto. i. *)
+(*             rewrite x0 in *. inv GET0. *)
+(*             eapply STABLE_MEM1; eauto. *)
+(*       } *)
+
+(*       { (* split *) *)
+(*         des. subst. *)
+(*         splits; ss. *)
+(*         - ii. revert GET. *)
+(*           erewrite Memory.split_o; eauto. repeat condtac; ss; i. *)
+(*           + des. subst. inv GET. *)
+(*             exploit MSG; eauto. i. des. eauto. *)
+(*           + guardH o. des. subst. inv GET. *)
+(*             exploit Memory.split_get0; try exact MEM. i. des. *)
+(*             eapply NORMAL_MEM1; eauto. *)
+(*           + eapply NORMAL_MEM1; eauto. *)
+(*         - inv STABLE_TVIEW1. econs; ss; ii; revert GET. *)
+(*           + erewrite Memory.split_o; eauto. repeat condtac; ss; i. *)
+(*             * des. subst. inv GET. *)
+(*               exploit Memory.split_get0; try exact MEM. i. des. *)
+(*               inv TVIEW1. specialize (REL0 loc0). inv REL0. *)
+(*               specialize (RLX loc). des. congr. *)
+(*             * guardH o. des. subst. inv GET. *)
+(*               exploit Memory.split_get0; try exact MEM. i. des. *)
+(*               eapply REL; eauto. *)
+(*             * eapply REL; eauto. *)
+(*           + erewrite Memory.split_o; eauto. repeat condtac; ss; i; eauto. *)
+(*             * des. subst. inv GET. *)
+(*               exploit Memory.split_get0; try exact MEM. i. des. *)
+(*               inv TVIEW1. inv CUR0. *)
+(*               specialize (RLX loc). des. congr. *)
+(*             * guardH o. des. subst. inv GET. *)
+(*               exploit Memory.split_get0; try exact MEM. i. des. eauto. *)
+(*           + erewrite Memory.split_o; eauto. repeat condtac; ss; i; eauto. *)
+(*             * des. subst. inv GET. *)
+(*               exploit Memory.split_get0; try exact MEM. i. des. *)
+(*               inv TVIEW1. inv ACQ0. *)
+(*               specialize (RLX loc). des. congr. *)
+(*             * guardH o. des. subst. inv GET. *)
+(*               exploit Memory.split_get0; try exact MEM. i. des. eauto. *)
+(*         - ii. revert GET. *)
+(*           erewrite Memory.split_o; eauto. repeat condtac; ss; i. *)
+(*           + guardH LOC. des. subst. inv GET. *)
+(*             exploit MSG; eauto. i. des. eauto. *)
+(*           + guardH LOC. guardH o. des. subst. inv GET. *)
+(*             exploit Memory.split_get0; try exact MEM. i. des. *)
+(*             inv MEM1. exploit CLOSED; try exact GET1. i. des. *)
+(*             inv MSG_CLOSED. inv CLOSED0. inv CLOSED1. *)
+(*             specialize (RLX loc1). des. *)
+(*             exploit Memory.split_get1; try exact RLX; eauto. i. des. *)
+(*             rewrite GET4 in *. inv GET0. *)
+(*             eapply STABLE_MEM1; eauto. *)
+(*           + guardH LOC. guardH o. guardH o0. *)
+(*             inv MEM1. exploit CLOSED; eauto. i. des. *)
+(*             inv MSG_CLOSED. inv CLOSED0. inv CLOSED1. *)
+(*             specialize (RLX loc1). des. *)
+(*             exploit Memory.split_get1; try exact RLX; eauto. i. des. *)
+(*             rewrite GET2 in *. inv GET0. *)
+(*             eapply STABLE_MEM1; eauto. *)
+(*       } *)
+
+(*       { (* lower *) *)
+(*         splits; ss. *)
+(*         - ii. revert GET. *)
+(*           erewrite Memory.lower_o; eauto. condtac; ss; i. *)
+(*           + des. subst. inv GET. *)
+(*             exploit MSG; eauto. i. des. eauto. *)
+(*           + eapply NORMAL_MEM1; eauto. *)
+(*         - inv STABLE_TVIEW1. econs; ss; ii; revert GET. *)
+(*           + erewrite Memory.lower_o; eauto. condtac; ss; i. *)
+(*             * des. subst. inv GET. *)
+(*               exploit Memory.lower_get0; try exact MEM. i. des. *)
+(*               inv MSG_LE. inv RELEASED. etrans; eauto. *)
+(*               eapply REL; eauto. *)
+(*             * eapply REL; eauto. *)
+(*           + erewrite Memory.lower_o; eauto. condtac; ss; i; eauto. *)
+(*             des. subst. inv GET. *)
+(*             exploit Memory.lower_get0; try exact MEM. i. des. *)
+(*             inv MSG_LE. inv RELEASED. etrans; eauto. *)
+(*           + erewrite Memory.lower_o; eauto. condtac; ss; i; eauto. *)
+(*             des. subst. inv GET. *)
+(*             exploit Memory.lower_get0; try exact MEM. i. des. *)
+(*             inv MSG_LE. inv RELEASED. etrans; eauto. *)
+(*         - ii. revert GET. *)
+(*           erewrite Memory.lower_o; eauto. condtac; ss; i. *)
+(*           + guardH LOC. des. subst. inv GET. *)
+(*             exploit MSG; eauto. i. des. eauto. *)
+(*           + guardH LOC. guardH o. inv MEM1. exploit CLOSED; eauto. i. des. *)
+(*             inv MSG_CLOSED. inv CLOSED0. inv CLOSED1. *)
+(*             specialize (RLX loc1). des. *)
+(*             exploit Memory.lower_get1; try exact RLX; eauto. i. des. *)
+(*             rewrite GET2 in *. inv GET0. inv MSG_LE. inv RELEASED. *)
+(*             etrans; eauto. *)
+(*             eapply STABLE_MEM1; eauto. *)
+(*       } *)
+
+(*       { (* cancel *) *)
+(*         splits; ss. *)
+(*         - ii. revert GET. *)
+(*           erewrite Memory.remove_o; eauto. condtac; ss; i. *)
+(*           eapply NORMAL_MEM1; eauto. *)
+(*         - inv STABLE_TVIEW1. econs; ss; ii; revert GET. *)
+(*           + erewrite Memory.remove_o; eauto. condtac; ss; i. *)
+(*             eapply REL; eauto. *)
+(*           + erewrite Memory.remove_o; eauto. condtac; ss; i; eauto. *)
+(*           + erewrite Memory.remove_o; eauto. condtac; ss; i; eauto. *)
+(*         - ii. revert GET. *)
+(*           erewrite Memory.remove_o; eauto. condtac; ss; i. *)
+(*           guardH LOC. guardH o. inv MEM1. exploit CLOSED; eauto. i. des. *)
+(*           inv MSG_CLOSED. inv CLOSED0. inv CLOSED1. *)
+(*           specialize (RLX loc1). des. *)
+(*           exploit Memory.remove_get1; try exact RLX; eauto. i. des. *)
+(*           { subst. exploit Memory.remove_get0; try exact MEM. i. des. congr. } *)
+(*           rewrite GET2 in *. inv GET0. *)
+(*           eapply STABLE_MEM1; eauto. *)
+(*       } *)
+(*     Qed. *)
+
+(*     Lemma promise_step *)
+(*           rels lc1 mem1 loc from to msg lc2 mem2 kind *)
+(*           (WF1: Local.wf lc1 mem1) *)
+(*           (MEM1: Memory.closed mem1) *)
+(*           (NORMAL_TVIEW1: normal_tview (Local.tview lc1)) *)
+(*           (NORMAL_MEM1: normal_memory mem1) *)
+(*           (STABLE_TVIEW1: stable_tview mem1 (Local.tview lc1)) *)
+(*           (STABLE_MEM1: stable_memory rels mem1) *)
+(*           (RELS_WF1: RelWrites.wf rels (Local.promises lc1) mem1) *)
+(*           (MSG: forall val released *)
+(*                   (MSG: msg = Message.concrete val (Some released)), *)
+(*               normal_view released /\ stable_view mem2 released) *)
+(*           (STEP: Local.promise_step lc1 mem1 loc from to msg lc2 mem2 kind): *)
+(*       <<NORMAL_TVIEW2: normal_tview (Local.tview lc2)>> /\ *)
+(*       <<NORMAL_MEM2: normal_memory mem2>> /\ *)
+(*       <<STABLE_TVIEW2: stable_tview mem2 (Local.tview lc2)>> /\ *)
+(*       <<STABLE_MEM2: stable_memory rels mem2>> /\ *)
+(*       <<RELS_WF2: RelWrites.wf rels (Local.promises lc2) mem2>>. *)
+(*     Proof. *)
+(*       inv STEP. exploit promise; try apply WF1; eauto. i. des. *)
+(*       splits; auto. ii. ss. *)
+(*       exploit RELS_WF1; eauto. i. des. split. *)
+(*       - inv PROMISE. *)
+(*         + erewrite Memory.add_o; eauto. condtac; ss. *)
+(*           des. subst. exploit Memory.add_get0; try exact MEM. i. des. congr. *)
+(*         + erewrite Memory.split_o; eauto. repeat condtac; ss. *)
+(*           * des. subst. exploit Memory.split_get0; try exact MEM. i. des. congr. *)
+(*           * guardH o. des. subst. *)
+(*             exploit Memory.split_get0; try exact PROMISES. i. des. congr. *)
+(*         + erewrite Memory.lower_o; eauto. condtac; ss. *)
+(*           des. subst. exploit Memory.lower_get0; try exact PROMISES. i. des. congr. *)
+(*         + erewrite Memory.remove_o; eauto. condtac; ss. *)
+(*       - destruct (Memory.op_kind_is_cancel kind) eqn:KIND. *)
+(*         + destruct kind; ss. inv PROMISE. *)
+(*           erewrite Memory.remove_o; eauto. condtac; ss; eauto. *)
+(*           des. subst. exploit Memory.remove_get0; try exact MEM. i. des. congr. *)
+(*         + exploit Memory.promise_get1; eauto. i. des. inv MSG_LE. eauto. *)
+(*     Qed. *)
+
+(*     Lemma read_step_loc_cur *)
+(*           rels lc1 mem1 loc to val released ord lc2 *)
+(*           (WF1: Local.wf lc1 mem1) *)
+(*           (MEM1: Memory.closed mem1) *)
+(*           (NORMAL_TVIEW1: normal_tview (Local.tview lc1)) *)
+(*           (NORMAL_MEM1: normal_memory mem1) *)
+(*           (STABLE_TVIEW1: stable_tview mem1 (Local.tview lc1)) *)
+(*           (STABLE_MEM1: stable_memory rels mem1) *)
+(*           (LOC: L loc) *)
+(*           (TO: to = (TView.cur (Local.tview lc1)).(View.rlx) loc) *)
+(*           (STEP: Local.read_step lc1 mem1 loc to val released ord lc2): *)
+(*       <<LC2: lc2 = lc1>>. *)
+(*     Proof. *)
+(*       unnw. inv STEP. destruct lc1. f_equal; ss. *)
+(*       unfold TView.read_tview. condtac; ss; [|condtac; [|destruct ord]; ss]. *)
+(*       - condtac; [|destruct ord]; ss. *)
+(*         destruct tview; ss. f_equal; ss. *)
+(*         + repeat rewrite View.le_join_l; ss. *)
+(*           * eapply View.singleton_ur_spec; try apply WF1. *)
+(*             inv NORMAL_TVIEW1. rewrite CUR; ss. refl. *)
+(*           * destruct released; try apply View.bot_spec. ss. *)
+(*             inv STABLE_TVIEW1. eauto. *)
+(*           * eapply View.singleton_ur_spec; try apply WF1. *)
+(*             inv NORMAL_TVIEW1. rewrite CUR; ss. refl. *)
+(*         + repeat rewrite View.le_join_l; ss. *)
+(*           * inv WF1. ss. inv TVIEW_WF. ss. etrans; eauto. *)
+(*             eapply View.singleton_ur_spec; ss. *)
+(*             inv NORMAL_TVIEW1. rewrite CUR0; ss. refl. *)
+(*           * inv WF1. ss. inv TVIEW_WF. ss. etrans; eauto. *)
+(*             destruct released; try apply View.bot_spec. ss. *)
+(*             inv STABLE_TVIEW1. eauto. *)
+(*           * inv WF1. ss. inv TVIEW_WF. ss. etrans; eauto. *)
+(*             eapply View.singleton_ur_spec; ss. *)
+(*             inv NORMAL_TVIEW1. rewrite CUR0; ss. refl. *)
+(*       - destruct tview; ss. f_equal; ss. *)
+(*         + repeat rewrite View.le_join_l; ss. *)
+(*           * eapply View.singleton_ur_spec; try apply WF1. *)
+(*             inv NORMAL_TVIEW1. rewrite CUR; ss. refl. *)
+(*           * destruct released; try apply View.bot_spec. *)
+(*           * eapply View.singleton_ur_spec; try apply WF1. *)
+(*             inv NORMAL_TVIEW1. rewrite CUR; ss. refl. *)
+(*         + repeat rewrite View.le_join_l; ss. *)
+(*           * inv WF1. ss. inv TVIEW_WF. ss. etrans; eauto. *)
+(*             eapply View.singleton_ur_spec; ss. *)
+(*             inv NORMAL_TVIEW1. rewrite CUR0; ss. refl. *)
+(*           * inv WF1. ss. inv TVIEW_WF. ss. etrans; eauto. *)
+(*             destruct released; try apply View.bot_spec. ss. *)
+(*             inv STABLE_TVIEW1. eauto. *)
+(*           * inv WF1. ss. inv TVIEW_WF. ss. etrans; eauto. *)
+(*             eapply View.singleton_ur_spec; ss. *)
+(*             inv NORMAL_TVIEW1. rewrite CUR0; ss. refl. *)
+(*       - destruct tview; ss. f_equal; ss. *)
+(*         + repeat rewrite View.le_join_l; ss. *)
+(*           * eapply View.singleton_rw_spec; try apply WF1. *)
+(*             inv NORMAL_TVIEW1. rewrite CUR; ss. refl. *)
+(*           * destruct released; try apply View.bot_spec. *)
+(*           * eapply View.singleton_rw_spec; try apply WF1. *)
+(*             inv NORMAL_TVIEW1. rewrite CUR; ss. refl. *)
+(*         + repeat rewrite View.le_join_l; ss. *)
+(*           * inv WF1. ss. inv TVIEW_WF. ss. etrans; eauto. *)
+(*             eapply View.singleton_rw_spec; ss. *)
+(*             inv NORMAL_TVIEW1. rewrite CUR0; ss. refl. *)
+(*           * inv WF1. ss. inv TVIEW_WF. ss. etrans; eauto. *)
+(*             destruct released; try apply View.bot_spec. *)
+(*           * inv WF1. ss. inv TVIEW_WF. ss. etrans; eauto. *)
+(*             eapply View.singleton_rw_spec; ss. *)
+(*             inv NORMAL_TVIEW1. rewrite CUR0; ss. refl. *)
+(*     Qed. *)
+
+(*     Lemma read_step_loc_ra *)
+(*           rels lc1 mem1 loc to val released ord lc2 *)
+(*           (WF1: Local.wf lc1 mem1) *)
+(*           (MEM1: Memory.closed mem1) *)
+(*           (NORMAL_TVIEW1: normal_tview (Local.tview lc1)) *)
+(*           (NORMAL_MEM1: normal_memory mem1) *)
+(*           (STABLE_TVIEW1: stable_tview mem1 (Local.tview lc1)) *)
+(*           (STABLE_MEM1: stable_memory rels mem1) *)
+(*           (RELS_WF1: RelWrites.wf rels (Local.promises lc1) mem1) *)
+(*           (LOC: L loc) *)
+(*           (REL: List.In (loc, to) rels) *)
+(*           (ORD: Ordering.le Ordering.acqrel ord) *)
+(*           (STEP: Local.read_step lc1 mem1 loc to val released ord lc2): *)
+(*       <<NORMAL_TVIEW2: normal_tview (Local.tview lc2)>> /\ *)
+(*       <<STABLE_TVIEW2: stable_tview mem1 (Local.tview lc2)>> /\ *)
+(*       <<RELS_WF2: RelWrites.wf rels (Local.promises lc2) mem1>>. *)
+(*     Proof. *)
+(*       inv STEP. ss. splits; ss. *)
+(*       - inv NORMAL_TVIEW1. econs; ss. *)
+(*         + repeat eapply join_normal_view; ss. *)
+(*           { destruct ord; ss. } *)
+(*           { condtac; ss. destruct released; ss; eauto. } *)
+(*         + repeat eapply join_normal_view; ss. *)
+(*           { destruct ord; ss. } *)
+(*           { condtac; ss. destruct released; ss; eauto. } *)
+(*       - inv STABLE_TVIEW1. econs; ss. *)
+(*         + unfold View.singleton_ur_if. *)
+(*           repeat (condtac; [|destruct ord; ss]). ii. *)
+(*           destruct (Loc.eq_dec loc loc0); subst; ss. *)
+(*           * unfold TimeMap.join, View.singleton_ur_if, *)
+(*             TimeMap.singleton, LocFun.add, LocFun.init, LocFun.find in GET0. *)
+(*             revert GET0. condtac; ss. i. *)
+(*             rewrite TimeFacts.le_join_l in GET0; cycle 1. *)
+(*             { etrans; [|eapply Time.join_r]. *)
+(*               inv MEM1. exploit CLOSED; try exact GET. i. des. *)
+(*               inv MSG_TS. ss. } *)
+(*             rewrite TimeFacts.le_join_r in GET0; cycle 1. *)
+(*             { inv READABLE. auto. } *)
+(*             rewrite GET0 in *. inv GET. ss. *)
+(*             etrans; [|apply View.join_r]. refl. *)
+(*           * unfold TimeMap.join, View.singleton_ur_if, *)
+(*             TimeMap.singleton, LocFun.add, LocFun.init, LocFun.find in GET0. *)
+(*             revert GET0. condtac; try congr; ss. i. *)
+(*             rewrite (@TimeFacts.le_join_l _ Time.bot) in GET0; try apply Time.bot_spec. *)
+(*             exploit Time.join_cases. i. des. *)
+(*             { rewrite x0 in GET0. *)
+(*               exploit CUR; eauto. i. etrans; eauto. *)
+(*               etrans; [|apply View.join_l]. *)
+(*               etrans; [|apply View.join_l]. *)
+(*               refl. } *)
+(*             { rewrite x0 in GET0. destruct released; ss; cycle 1. *)
+(*               { unfold TimeMap.bot in *. *)
+(*                 inv MEM1. rewrite INHABITED in GET0. ss. } *)
+(*               exploit STABLE_MEM1; try exact GET; eauto. i. *)
+(*               etrans; eauto. *)
+(*               etrans; [|apply View.join_r]. *)
+(*               refl. } *)
+(*         + unfold View.singleton_ur_if. *)
+(*           repeat (condtac; [|destruct ord; ss]). ii. *)
+(*           destruct (Loc.eq_dec loc loc0); subst; ss. *)
+(*           * unfold TimeMap.join, View.singleton_ur_if, *)
+(*             TimeMap.singleton, LocFun.add, LocFun.init, LocFun.find in GET0. *)
+(*             revert GET0. condtac; ss. i. *)
+(*             rewrite Time.join_assoc in GET0. *)
+(*             rewrite (@TimeFacts.le_join_l to) in GET0; cycle 1. *)
+(*             { inv MEM1. exploit CLOSED; try exact GET. i. des. *)
+(*               inv MSG_TS. ss. } *)
+(*             exploit Time.join_cases. i. des. *)
+(*             { rewrite x0 in GET0. *)
+(*               exploit ACQ; eauto. i. etrans; eauto. *)
+(*               etrans; [|apply View.join_l]. *)
+(*               etrans; [|apply View.join_l]. *)
+(*               refl. } *)
+(*             { rewrite x0 in GET0. rewrite GET0 in *. inv GET. ss. *)
+(*               etrans; [|apply View.join_r].  *)
+(*               refl. } *)
+(*           * unfold TimeMap.join, View.singleton_ur_if, *)
+(*             TimeMap.singleton, LocFun.add, LocFun.init, LocFun.find in GET0. *)
+(*             revert GET0. condtac; try congr; ss. i. *)
+(*             rewrite (@TimeFacts.le_join_l _ Time.bot) in GET0; try apply Time.bot_spec. *)
+(*             exploit Time.join_cases. i. des. *)
+(*             { rewrite x0 in GET0. *)
+(*               exploit ACQ; eauto. i. etrans; eauto. *)
+(*               etrans; [|apply View.join_l]. *)
+(*               etrans; [|apply View.join_l]. *)
+(*               refl. } *)
+(*             { rewrite x0 in GET0. destruct released; ss; cycle 1. *)
+(*               { unfold TimeMap.bot in *. *)
+(*                 inv MEM1. rewrite INHABITED in GET0. ss. } *)
+(*               exploit STABLE_MEM1; try exact GET; eauto. i. *)
+(*               etrans; eauto. *)
+(*               etrans; [|apply View.join_r]. *)
+(*               refl. } *)
+(*     Qed. *)
+
+(*     Lemma read_step_other *)
+(*           rels lc1 mem1 loc to val released ord lc2 *)
+(*           (WF1: Local.wf lc1 mem1) *)
+(*           (MEM1: Memory.closed mem1) *)
+(*           (NORMAL_TVIEW1: normal_tview (Local.tview lc1)) *)
+(*           (NORMAL_MEM1: normal_memory mem1) *)
+(*           (STABLE_TVIEW1: stable_tview mem1 (Local.tview lc1)) *)
+(*           (STABLE_MEM1: stable_memory rels mem1) *)
+(*           (RELS_WF1: RelWrites.wf rels (Local.promises lc1) mem1) *)
+(*           (LOC: ~ L loc) *)
+(*           (STEP: Local.read_step lc1 mem1 loc to val released ord lc2): *)
+(*       <<NORMAL_TVIEW2: normal_tview (Local.tview lc2)>> /\ *)
+(*       <<STABLE_TVIEW2: stable_tview mem1 (Local.tview lc2)>> /\ *)
+(*       <<RELS_WF2: RelWrites.wf rels (Local.promises lc2) mem1>>. *)
+(*     Proof. *)
+(*       inv STEP. ss. splits; ss. *)
+(*       - inv NORMAL_TVIEW1. econs; ss. *)
+(*         + repeat apply join_normal_view; ss. *)
+(*           * apply singleton_ur_if_normal_view. ss. *)
+(*           * condtac; ss. destruct released; ss. eauto. *)
+(*         + repeat apply join_normal_view; ss. *)
+(*           * apply singleton_ur_if_normal_view. ss. *)
+(*           * condtac; ss. destruct released; ss. eauto. *)
+(*       - inv STABLE_TVIEW1. econs; ss. *)
+(*         + repeat apply join_stable_view; ss. *)
+(*           * apply singleton_ur_if_stable_view; ss. *)
+(*           * condtac; ss. *)
+(*             { destruct released; ss. *)
+(*               - eapply STABLE_MEM1; eauto. *)
+(*               - apply bot_stable_view; ss. } *)
+(*             { apply bot_stable_view; ss. } *)
+(*         + repeat apply join_stable_view; ss. *)
+(*           * apply singleton_ur_if_stable_view; ss. *)
+(*           * condtac; ss. *)
+(*             { destruct released; ss. *)
+(*               - eapply STABLE_MEM1; eauto. *)
+(*               - apply bot_stable_view; ss. } *)
+(*             { apply bot_stable_view; ss. } *)
+(*     Qed. *)
+
+(*     Lemma write_step_loc *)
+(*           rels lc1 sc1 mem1 loc from to val releasedm released ord lc2 sc2 mem2 kind *)
+(*           (WF1: Local.wf lc1 mem1) *)
+(*           (SC1: Memory.closed_timemap sc1 mem1) *)
+(*           (MEM1: Memory.closed mem1) *)
+(*           (RELS_WF1: RelWrites.wf rels (Local.promises lc1) mem1) *)
+(*           (NORMAL_TVIEW1: normal_tview (Local.tview lc1)) *)
+(*           (NORMAL_MEM1: normal_memory mem1) *)
+(*           (STABLE_TVIEW1: stable_tview mem1 (Local.tview lc1)) *)
+(*           (STABLE_MEM1: stable_memory rels mem1) *)
+(*           (WF_RELEASEDM: View.opt_wf releasedm) *)
+(*           (CLOSED_RELEASEDM: Memory.closed_opt_view releasedm mem1) *)
+(*           (NORMAL_RELEASEDM: normal_view (View.unwrap releasedm)) *)
+(*           (RELEASEDM: View.le (View.unwrap releasedm) (TView.cur (Local.tview lc1))) *)
+(*           (LOC: L loc) *)
+(*           (STEP: Local.write_step lc1 sc1 mem1 loc from to val releasedm released ord lc2 sc2 mem2 kind): *)
+(*       <<NORMAL_TVIEW2: normal_tview (Local.tview lc2)>> /\ *)
+(*       <<NORMAL_MEM2: normal_memory mem2>> /\ *)
+(*       <<STABLE_TVIEW2: stable_tview mem2 (Local.tview lc2)>> /\ *)
+(*       <<STABLE_MEM2: stable_memory (if Ordering.le Ordering.acqrel ord then (loc, to) :: rels else rels) mem2>> /\ *)
+(*       <<RELS_WF2: RelWrites.wf (if Ordering.le Ordering.acqrel ord then (loc, to) :: rels else rels)  *)
+(*                                    (Local.promises lc2) mem2>>. *)
+(*     Proof. *)
+(*       exploit Local.write_step_future; eauto. i. des. *)
+(*       inv STEP. inv WRITE. ss. *)
+(*       assert (NORMAL_TVIEW2: normal_tview (TView.write_tview (Local.tview lc1) sc1 loc to ord)). *)
+(*       { inv NORMAL_TVIEW1. *)
+(*         econs; ss; i; try by (apply join_normal_view; ss). *)
+(*         unfold LocFun.add. condtac; eauto. subst. *)
+(*         condtac; apply join_normal_view; ss. } *)
+(*       assert (STABLE_TVIEW2: stable_tview mem2 (TView.write_tview (Local.tview lc1) sc1 loc to ord)). *)
+(*       { inv STABLE_TVIEW1. econs; ss; i. *)
+(*         - condtac; ss. *)
+(*           { unfold LocFun.add, LocFun.find. *)
+(*             condtac; ss; subst; ii; ss. *)
+(*             inv WF1. inv TVIEW_WF. inv TVIEW_CLOSED. *)
+(*             destruct (REL1 loc0). specialize (RLX loc1). des. *)
+(*             exploit Memory.promise_get1; try exact RLX; eauto. *)
+(*             { inv PROMISE; ss. } *)
+(*             i. des. *)
+(*             rewrite GET0 in *. inv GET. inv MSG_LE. inv RELEASED. *)
+(*             etrans; eauto. eapply REL; eauto. *)
+(*           } *)
+(*           { unfold LocFun.add, LocFun.find. *)
+(*             condtac; ss; subst; ii; ss. *)
+(*             inv WF1. inv TVIEW_WF. inv TVIEW_CLOSED. *)
+(*             destruct (REL1 loc0). specialize (RLX loc1). des. *)
+(*             exploit Memory.promise_get1; try exact RLX; eauto. *)
+(*             { inv PROMISE; ss. } *)
+(*             i. des. *)
+(*             rewrite GET0 in *. inv GET. inv MSG_LE. inv RELEASED. *)
+(*             etrans; eauto. eapply REL; eauto. *)
+(*           } *)
+(*         - ii. revert GET. ss. *)
+(*           unfold TimeMap.join, TimeMap.singleton, LocFun.add, LocFun.init, LocFun.find. *)
+(*           condtac; ss; subst; i. *)
+(*           + rewrite TimeFacts.le_join_r in GET; cycle 1. *)
+(*             { inv WRITABLE. econs. ss. } *)
+(*             exploit Memory.promise_get0; try exact PROMISE. *)
+(*             { inv PROMISE; ss. } *)
+(*             i. des. *)
+(*             rewrite GET in *. inv GET_MEM. *)
+(*             revert H2. unfold TView.write_released. condtac; ss. *)
+(*             unfold LocFun.add. repeat condtac; ss. *)
+(*             * i. inv H2. *)
+(*               repeat eapply View.join_spec; eauto using View.join_l, View.join_r. *)
+(*             * i. inv H2. *)
+(*               repeat eapply View.join_spec; eauto using View.join_l, View.join_r. *)
+(*               etrans; try eapply WF1. apply View.join_l. *)
+(*           + rewrite TimeFacts.le_join_l in GET; try by apply Time.bot_spec. *)
+(*             etrans; [|apply View.join_l]. *)
+(*             revert GET. inv PROMISE. *)
+(*             { erewrite Memory.add_o; eauto. condtac; ss; i; eauto. *)
+(*               des. subst. inv GET. ss. } *)
+(*             { erewrite Memory.split_o; eauto. repeat condtac; ss; i; eauto. *)
+(*               - des. subst. inv GET. ss. *)
+(*               - guardH o. des. subst. inv GET. ss. } *)
+(*             { erewrite Memory.lower_o; eauto. condtac; ss; i; eauto. *)
+(*               des. subst. inv GET. ss. } *)
+(*             { exploit Memory.remove_get0; try exact PROMISES. i. des. *)
+(*               exploit Memory.remove_get0; try exact REMOVE. i. des. *)
+(*               congr. } *)
+(*         - ii.  revert GET. ss. *)
+(*           unfold TimeMap.join, TimeMap.singleton, LocFun.add, LocFun.init, LocFun.find. *)
+(*           condtac; ss; subst; i. *)
+(*           + exploit Time.join_cases. i. des. *)
+(*             * erewrite x0 in GET. *)
+(*               inv WF1. inv TVIEW_CLOSED. inv ACQ0. *)
+(*               destruct (RLX loc). des. *)
+(*               exploit Memory.promise_get1; try exact H; eauto. *)
+(*               { inv PROMISE; ss. } *)
+(*               i. des. *)
+(*               rewrite GET0 in *. inv GET. inv MSG_LE. inv RELEASED. *)
+(*               etrans; eauto. *)
+(*               etrans; [|apply View.join_l]. *)
+(*               eauto. *)
+(*             * erewrite x0 in GET. *)
+(*               exploit Memory.promise_get0; try exact PROMISE. *)
+(*               { inv PROMISE; ss. } *)
+(*               i. des. *)
+(*               rewrite GET in *. inv GET_MEM. *)
+(*               revert H2. unfold TView.write_released. condtac; ss. *)
+(*               unfold LocFun.add. repeat condtac; ss. *)
+(*               { i. inv H2. *)
+(*                 repeat eapply View.join_spec; try apply View.join_r. *)
+(*                 - etrans; eauto. *)
+(*                   etrans; try eapply WF1. apply View.join_l. *)
+(*                 - etrans; try eapply WF1. apply View.join_l. } *)
+(*               { i. inv H2. *)
+(*                 repeat eapply View.join_spec; try apply View.join_r. *)
+(*                 - etrans; eauto. *)
+(*                   etrans; try eapply WF1. apply View.join_l. *)
+(*                 - etrans; try eapply WF1. etrans; try eapply WF1. apply View.join_l. } *)
+(*           + rewrite TimeFacts.le_join_l in GET; try by apply Time.bot_spec. *)
+(*             etrans; [|apply View.join_l]. *)
+(*             revert GET. inv PROMISE. *)
+(*             { erewrite Memory.add_o; eauto. condtac; ss; i; eauto. *)
+(*               des. subst. inv GET. ss. } *)
+(*             { erewrite Memory.split_o; eauto. repeat condtac; ss; i; eauto. *)
+(*               - des. subst. inv GET. ss. *)
+(*               - guardH o. des. subst. inv GET. ss. } *)
+(*             { erewrite Memory.lower_o; eauto. condtac; ss; i; eauto. *)
+(*               des. subst. inv GET. ss. } *)
+(*             { exploit Memory.remove_get0; try exact PROMISES. i. des. *)
+(*               exploit Memory.remove_get0; try exact REMOVE. i. des. *)
+(*               congr. } *)
+(*       } *)
+
+(*       assert (NORMAL_RELEASED: forall released, *)
+(*                  TView.write_released (Local.tview lc1) sc1 loc to releasedm ord = Some released -> *)
+(*                  normal_view released). *)
+(*       { unfold TView.write_released. repeat (condtac; ss). *)
+(*         unfold LocFun.add. condtac; ss. *)
+(*         - i. inv H. repeat apply join_normal_view; ss. apply NORMAL_TVIEW1. *)
+(*         - i. inv H. unfold LocFun.add. condtac; ss. *)
+(*           repeat apply join_normal_view; ss. apply NORMAL_TVIEW1. } *)
+
+(*       condtac; ss. *)
+(*       { assert (RELEASED: TView.write_released (Local.tview lc1) sc1 loc to releasedm ord = *)
+(*                           Some (View.join (View.singleton_ur loc to) (TView.cur (Local.tview lc1)))). *)
+(*         { unfold TView.write_released. repeat (condtac; ss); cycle 1. *)
+(*           { destruct ord; ss. } *)
+(*           f_equal. *)
+(*           unfold LocFun.add. condtac; ss. *)
+(*           rewrite (View.join_comm (View.singleton_ur loc to)). *)
+(*           apply View.antisym; cycle 1. *)
+(*           { etrans; [|eapply View.join_r]. refl. } *)
+(*           apply View.join_spec; try refl. *)
+(*           etrans; [|eapply View.join_l]. ss. *)
+(*         } *)
+(*         assert (STABLE_RELEASED: *)
+(*                   stable_view mem2 (View.join (View.singleton_ur loc to) (TView.cur (Local.tview lc1)))). *)
+(*         { rewrite RELEASED in *. ii. revert GET. ss. *)
+(*           unfold TimeMap.join, TimeMap.singleton, LocFun.add, LocFun.init, LocFun.find. condtac; ss. *)
+(*           - subst. replace (Time.join to (View.rlx (TView.cur (Local.tview lc1)) loc)) with to; cycle 1. *)
+(*             { rewrite TimeFacts.le_join_l; ss. *)
+(*               inv WRITABLE. econs. ss. } *)
+(*             exploit Memory.promise_get0; try exact PROMISE; try by (inv PROMISE; ss). i. des. *)
+(*             rewrite GET_MEM in *. inv GET. refl. *)
+(*           - rewrite TimeFacts.le_join_r; try by apply Time.bot_spec. i. *)
+(*             inv WF1. inv TVIEW_CLOSED. inv CUR. specialize (RLX loc0). des. *)
+(*             exploit Memory.promise_get1; try exact RLX; eauto; try by (inv PROMISE; ss). i. des. *)
+(*             rewrite GET0 in *. inv GET. inv MSG_LE. inv RELEASED0. *)
+(*             etrans; eauto. etrans; [|apply View.join_r]. *)
+(*             eapply STABLE_TVIEW1; eauto. *)
+(*         } *)
+(*         exploit promise; try exact PROMISE; try apply WF1; eauto. *)
+(*         { i. inv MSG. rewrite RELEASED in *. inv H1. split; ss. *)
+(*           apply join_normal_view. *)
+(*           eauto using singleton_ur_normal_view. *)
+(*           apply NORMAL_TVIEW1. } *)
+(*         i. des. splits; auto. *)
+(*         - ii. ss. des. *)
+(*           + eapply STABLE_MEM2; eauto. *)
+(*           + inv LOC0. exploit Memory.promise_get0; try exact PROMISE; try by (inv PROMISE; ss). i. des. *)
+(*             rewrite GET in *. inv GET_MEM. *)
+(*             rewrite RELEASED in *. inv H2. *)
+(*             eapply STABLE_RELEASED; eauto. *)
+(*           + eapply STABLE_MEM2; eauto. *)
+(*         - ii. ss. des. *)
+(*           + inv IN. exploit Memory.promise_get2; eauto; try by (inv PROMISE; ss). i. des. *)
+(*             exploit Memory.remove_get0; eauto. i. des. eauto. *)
+(*           + exploit RELS_WF1; eauto. i. des. *)
+(*             exploit Memory.promise_get1; try exact x0; eauto; try by (inv PROMISE; ss). i. des. *)
+(*             inv MSG_LE. esplits; eauto. *)
+(*             erewrite Memory.remove_o; eauto. condtac; ss. *)
+(*             guardH o. inv PROMISE; ss. *)
+(*             * erewrite Memory.add_o; eauto. condtac; ss. *)
+(*             * erewrite Memory.split_o; eauto. repeat condtac; ss. *)
+(*               guardH o0. des. subst. *)
+(*               exploit Memory.split_get0; try exact PROMISES. i. des. congr. *)
+(*             * erewrite Memory.lower_o; eauto. condtac; ss. *)
+(*       } *)
+
+(*       splits; auto. *)
+(*       - ii. revert GET. inv PROMISE; ss. *)
+(*         + erewrite Memory.add_o; eauto. condtac; ss. *)
+(*           * i. des. subst. inv GET. *)
+(*             eapply NORMAL_RELEASED; eauto. *)
+(*           * i. eapply NORMAL_MEM1; eauto. *)
+(*         + erewrite Memory.split_o; eauto. repeat condtac; ss. *)
+(*           * i. des. subst. inv GET. *)
+(*             eapply NORMAL_RELEASED; eauto. *)
+(*           * guardH o. des. subst. i. inv GET. *)
+(*             exploit Memory.split_get0; try exact MEM. i. des. *)
+(*             eapply NORMAL_MEM1; eauto. *)
+(*           * i. eapply NORMAL_MEM1; eauto. *)
+(*         + erewrite Memory.lower_o; eauto. condtac; ss. *)
+(*           * i. des. subst. inv GET. *)
+(*             eapply NORMAL_RELEASED; eauto. *)
+(*           * i. eapply NORMAL_MEM1; eauto. *)
+(*       - ii. guardH LOC0. revert GET. inv PROMISE; ss. *)
+(*         + erewrite Memory.add_o; eauto. condtac; ss. *)
+(*           * i. des. subst. inv GET. unguard. des; ss. subst. *)
+(*             exploit RELS_WF1; eauto. i. des. *)
+(*             exploit Memory.add_get0; try exact MEM. i. des. congr. *)
+(*           * guardH o. i. inv MEM1. exploit CLOSED; eauto. i. des. *)
+(*             inv MSG_CLOSED. inv CLOSED0. inv CLOSED1. *)
+(*             specialize (RLX loc1). des. *)
+(*             exploit Memory.add_get1; try exact RLX; eauto. i. *)
+(*             rewrite x0 in *. inv GET0. eapply STABLE_MEM1; eauto. *)
+(*         + erewrite Memory.split_o; eauto. repeat condtac; ss. *)
+(*           * i. des. subst. inv GET. unguard. des; ss. *)
+(*             exploit RELS_WF1; eauto. i. des. *)
+(*             exploit Memory.split_get0; try exact MEM. i. des. congr. *)
+(*           * guardH o. i. des. subst. inv GET. *)
+(*             exploit Memory.split_get0; try exact MEM. i. des. *)
+(*             inv MEM1. exploit CLOSED; try exact GET1. i. des. *)
+(*             inv MSG_CLOSED. inv CLOSED0. inv CLOSED1. *)
+(*             specialize (RLX loc1). des. *)
+(*             exploit Memory.split_get1; try exact RLX; eauto. i. des. *)
+(*             rewrite GET4 in *. inv GET0. *)
+(*             eapply STABLE_MEM1; eauto. *)
+(*           * guardH o. guardH o0. i. *)
+(*             inv MEM1. exploit CLOSED; eauto. i. des. *)
+(*             inv MSG_CLOSED. inv CLOSED0. inv CLOSED1. *)
+(*             specialize (RLX loc1). des. *)
+(*             exploit Memory.split_get1; try exact RLX; eauto. i. des. *)
+(*             rewrite GET2 in *. inv GET0. eapply STABLE_MEM1; eauto. *)
+(*         + erewrite Memory.lower_o; eauto. condtac; ss. *)
+(*           * i. des. subst. inv GET. unguard. des; ss. *)
+(*             exploit RELS_WF1; eauto. i. des. *)
+(*             exploit Memory.lower_get0; try exact PROMISES. i. des. congr. *)
+(*           * guardH o. i. inv MEM1. exploit CLOSED; eauto. i. des. *)
+(*             inv MSG_CLOSED. inv CLOSED0. inv CLOSED1. *)
+(*             specialize (RLX loc1). des. *)
+(*             exploit Memory.lower_get1; try exact RLX; eauto. i. des. inv MSG_LE. *)
+(*             rewrite GET2 in *. inv GET0. inv RELEASED. *)
+(*             etrans; eauto. eapply STABLE_MEM1; eauto. *)
+(*       - ii. ss. exploit RELS_WF1; eauto. i. des. *)
+(*         exploit Memory.promise_get1; try exact x0; eauto; try by (inv PROMISE; ss). i. des. *)
+(*         inv MSG_LE. esplits; eauto. *)
+(*         erewrite Memory.remove_o; eauto. condtac; ss. guardH o. *)
+(*         inv PROMISE; ss. *)
+(*         + erewrite Memory.add_o; eauto. condtac; ss. *)
+(*         + erewrite Memory.split_o; eauto. repeat condtac; ss. *)
+(*           guardH o0. des. subst. *)
+(*           exploit Memory.split_get0; try exact PROMISES. i. des. congr. *)
+(*         + erewrite Memory.lower_o; eauto. condtac; ss. *)
+(*     Qed. *)
+
+(*     Lemma write_step_loc_None *)
+(*           rels lc1 sc1 mem1 loc from to val released ord lc2 sc2 mem2 kind *)
+(*           (WF1: Local.wf lc1 mem1) *)
+(*           (SC1: Memory.closed_timemap sc1 mem1) *)
+(*           (MEM1: Memory.closed mem1) *)
+(*           (NORMAL_TVIEW1: normal_tview (Local.tview lc1)) *)
+(*           (NORMAL_MEM1: normal_memory mem1) *)
+(*           (STABLE_TVIEW1: stable_tview mem1 (Local.tview lc1)) *)
+(*           (STABLE_MEM1: stable_memory rels mem1) *)
+(*           (RELS_WF1: RelWrites.wf rels (Local.promises lc1) mem1) *)
+(*           (LOC: L loc) *)
+(*           (STEP: Local.write_step lc1 sc1 mem1 loc from to val None released ord lc2 sc2 mem2 kind): *)
+(*       <<NORMAL_TVIEW2: normal_tview (Local.tview lc2)>> /\ *)
+(*       <<NORMAL_MEM2: normal_memory mem2>> /\ *)
+(*       <<STABLE_TVIEW2: stable_tview mem2 (Local.tview lc2)>> /\ *)
+(*       <<STABLE_MEM2: stable_memory (if Ordering.le Ordering.acqrel ord then (loc, to) :: rels else rels) mem2>> /\ *)
+(*       <<RELS_WF2: RelWrites.wf (if Ordering.le Ordering.acqrel ord then (loc, to) :: rels else rels)  *)
+(*                                    (Local.promises lc2) mem2>>. *)
+(*     Proof. *)
+(*       eapply write_step_loc; eauto; ss. *)
+(*       - apply View.bot_spec. *)
+(*     Qed. *)
+
+(*     Lemma write_step_other *)
+(*           rels lc1 sc1 mem1 loc from to val releasedm released ord lc2 sc2 mem2 kind *)
+(*           (WF1: Local.wf lc1 mem1) *)
+(*           (SC1: Memory.closed_timemap sc1 mem1) *)
+(*           (MEM1: Memory.closed mem1) *)
+(*           (NORMAL_TVIEW1: normal_tview (Local.tview lc1)) *)
+(*           (NORMAL_MEM1: normal_memory mem1) *)
+(*           (STABLE_TVIEW1: stable_tview mem1 (Local.tview lc1)) *)
+(*           (STABLE_MEM1: stable_memory rels mem1) *)
+(*           (RELS_WF1: RelWrites.wf rels (Local.promises lc1) mem1) *)
+(*           (LOC: ~ L loc) *)
+(*           (WF_RELEASEDM: View.opt_wf releasedm) *)
+(*           (CLOSED_RELEASEDM: Memory.closed_opt_view releasedm mem1) *)
+(*           (NORMAL_RELEASEDM: normal_view (View.unwrap releasedm)) *)
+(*           (STABLE_RELEASEDM: stable_view mem1 (View.unwrap releasedm)) *)
+(*           (STEP: Local.write_step lc1 sc1 mem1 loc from to val releasedm released ord lc2 sc2 mem2 kind): *)
+(*       <<NORMAL_TVIEW2: normal_tview (Local.tview lc2)>> /\ *)
+(*       <<NORMAL_MEM2: normal_memory mem2>> /\ *)
+(*       <<STABLE_TVIEW2: stable_tview mem2 (Local.tview lc2)>> /\ *)
+(*       <<STABLE_MEM2: stable_memory rels mem2>> /\ *)
+(*       <<RELS_WF2: RelWrites.wf rels (Local.promises lc2) mem2>>. *)
+(*     Proof. *)
+(*       exploit Local.write_step_future; eauto. i. des. *)
+(*       inv STEP. inv WRITE. ss. *)
+(*       assert (NORMAL_TVIEW2: normal_tview (TView.write_tview (Local.tview lc1) sc1 loc to ord)). *)
+(*       { inv NORMAL_TVIEW1. *)
+(*         econs; ss; i; try by (apply join_normal_view; ss). *)
+(*         unfold LocFun.add. condtac; eauto. subst. *)
+(*         condtac; apply join_normal_view; ss. } *)
+(*       assert (STABLE_TVIEW2: stable_tview mem2 (TView.write_tview (Local.tview lc1) sc1 loc to ord)). *)
+(*       { inv STABLE_TVIEW1. econs; ss; i. *)
+(*         { condtac; ss. *)
+(*           - unfold LocFun.add, LocFun.find. *)
+(*             condtac; ss; subst; ii; ss. *)
+(*             + revert GET. *)
+(*               unfold TimeMap.join, TimeMap.singleton, LocFun.add, LocFun.init, LocFun.find. *)
+(*               condtac; ss; i. *)
+(*               * subst. congr. *)
+(*               * rewrite TimeFacts.le_join_l in GET; try by apply Time.bot_spec. *)
+(*                 etrans; [|eapply View.join_l]. *)
+(*                 revert GET. inv PROMISE. *)
+(*                 { erewrite Memory.add_o; eauto. condtac; ss; i; eauto. *)
+(*                   des. subst. inv GET. ss. } *)
+(*                 { erewrite Memory.split_o; eauto. repeat condtac; ss; i; eauto. *)
+(*                   - des. subst. inv GET. ss. *)
+(*                   - guardH o. des. subst. inv GET. ss. } *)
+(*                 { erewrite Memory.lower_o; eauto. condtac; ss; i; eauto. *)
+(*                   des. subst. inv GET. ss. } *)
+(*                 { exploit Memory.remove_get0; try exact PROMISES. i. des. *)
+(*                   exploit Memory.remove_get0; try exact REMOVE. i. des. *)
+(*                   congr. } *)
+(*             + inv WF1. inv TVIEW_WF. inv TVIEW_CLOSED. *)
+(*               destruct (REL1 loc0). specialize (RLX loc1). des. *)
+(*               exploit Memory.promise_get1; try exact RLX; eauto. *)
+(*               { inv PROMISE; ss. } *)
+(*               i. des. *)
+(*               rewrite GET0 in *. inv GET. inv MSG_LE. inv RELEASED. *)
+(*               etrans; eauto. eapply REL; eauto. *)
+(*           - unfold LocFun.add, LocFun.find. *)
+(*             condtac; ss; subst; ii; ss. *)
+(*             + revert GET. *)
+(*               unfold TimeMap.join, TimeMap.singleton, LocFun.add, LocFun.init, LocFun.find. *)
+(*               condtac; ss; i. *)
+(*               * subst. congr. *)
+(*               * rewrite TimeFacts.le_join_l in GET; try by apply Time.bot_spec. *)
+(*                 etrans; [|eapply View.join_l]. *)
+(*                 revert GET. inv PROMISE. *)
+(*                 { erewrite Memory.add_o; eauto. condtac; ss; i. *)
+(*                   - des. subst. inv GET. ss. *)
+(*                   - eapply REL; eauto. } *)
+(*                 { erewrite Memory.split_o; eauto. repeat condtac; ss; i; eauto. *)
+(*                   - des. subst. inv GET. ss. *)
+(*                   - guardH o. des. subst. inv GET. ss. *)
+(*                   - eapply REL; eauto. } *)
+(*                 { erewrite Memory.lower_o; eauto. condtac; ss; i. *)
+(*                   - des. subst. inv GET. ss. *)
+(*                   - eapply REL; eauto. } *)
+(*                 { exploit Memory.remove_get0; try exact PROMISES. i. des. *)
+(*                   exploit Memory.remove_get0; try exact REMOVE. i. des. *)
+(*                   congr. } *)
+(*             + inv WF1. inv TVIEW_WF. inv TVIEW_CLOSED. *)
+(*               destruct (REL1 loc0). specialize (RLX loc1). des. *)
+(*               exploit Memory.promise_get1; try exact RLX; eauto. *)
+(*               { inv PROMISE; ss. } *)
+(*               i. des. *)
+(*               rewrite GET0 in *. inv GET. inv MSG_LE. inv RELEASED. *)
+(*               etrans; eauto. eapply REL; eauto. *)
+(*         } *)
+(*         { ii. revert GET. ss. *)
+(*           unfold TimeMap.join, TimeMap.singleton, LocFun.add, LocFun.init, LocFun.find. *)
+(*           condtac; ss; subst; i; try congr. *)
+(*           rewrite TimeFacts.le_join_l in GET; try by apply Time.bot_spec. *)
+(*           etrans; [|apply View.join_l]. *)
+(*           revert GET. inv PROMISE. *)
+(*           { erewrite Memory.add_o; eauto. condtac; ss; i; eauto. *)
+(*             des. subst. inv GET. ss. } *)
+(*           { erewrite Memory.split_o; eauto. repeat condtac; ss; i; eauto. *)
+(*             - des. subst. inv GET. ss. *)
+(*             - guardH o. des. subst. inv GET. ss. } *)
+(*           { erewrite Memory.lower_o; eauto. condtac; ss; i; eauto. *)
+(*             des. subst. inv GET. ss. } *)
+(*           { exploit Memory.remove_get0; try exact PROMISES. i. des. *)
+(*             exploit Memory.remove_get0; try exact REMOVE. i. des. *)
+(*             congr. } *)
+(*         } *)
+(*         { ii.  revert GET. ss. *)
+(*           unfold TimeMap.join, TimeMap.singleton, LocFun.add, LocFun.init, LocFun.find. *)
+(*           condtac; ss; subst; i; try congr. *)
+(*           rewrite TimeFacts.le_join_l in GET; try by apply Time.bot_spec. *)
+(*           etrans; [|apply View.join_l]. *)
+(*           revert GET. inv PROMISE. *)
+(*           { erewrite Memory.add_o; eauto. condtac; ss; i; eauto. *)
+(*             des. subst. inv GET. ss. } *)
+(*           { erewrite Memory.split_o; eauto. repeat condtac; ss; i; eauto. *)
+(*             - des. subst. inv GET. ss. *)
+(*             - guardH o. des. subst. inv GET. ss. } *)
+(*           { erewrite Memory.lower_o; eauto. condtac; ss; i; eauto. *)
+(*             des. subst. inv GET. ss. } *)
+(*           { exploit Memory.remove_get0; try exact PROMISES. i. des. *)
+(*             exploit Memory.remove_get0; try exact REMOVE. i. des. *)
+(*             congr. } *)
+(*         } *)
+(*       } *)
+
+(*       exploit promise; try exact PROMISE; try apply WF1; eauto. *)
+(*       { unfold TView.write_released. repeat (condtac; ss). *)
+(*         - unfold LocFun.add. condtac; ss. *)
+(*           i. inv MSG. split. *)
+(*           + repeat apply join_normal_view; ss. apply NORMAL_TVIEW1. *)
+(*           + ii. revert GET. *)
+(*             destruct (Loc.eq_dec loc loc0); subst; try congr. *)
+(*             ss. unfold TimeMap.join, TimeMap.singleton, LocFun.add, LocFun.init, LocFun.find. *)
+(*             condtac; ss; try congr. *)
+(*             rewrite (@TimeFacts.le_join_l _ Time.bot); try by apply Time.bot_spec. i. *)
+(*             rewrite <- View.join_assoc. *)
+(*             etrans; [|apply View.join_l]. *)
+(*             eapply future_stable_view; try eapply GET; try eapply join_stable_view; eauto. *)
+(*             * eapply Memory.join_closed_view; ss. *)
+(*               { inv CLOSED_RELEASEDM; ss. *)
+(*                 apply Memory.closed_view_bot. apply MEM1. } *)
+(*               { apply WF1. } *)
+(*             * apply STABLE_TVIEW1. *)
+(*         - unfold LocFun.add. condtac; ss. *)
+(*           i. inv MSG. split. *)
+(*           + repeat apply join_normal_view; ss. apply NORMAL_TVIEW1. *)
+(*           + ii. revert GET. *)
+(*             destruct (Loc.eq_dec loc loc0); subst; try congr. *)
+(*             ss. unfold TimeMap.join, TimeMap.singleton, LocFun.add, LocFun.init, LocFun.find. *)
+(*             condtac; ss; try congr. *)
+(*             rewrite (@TimeFacts.le_join_l _ Time.bot); try by apply Time.bot_spec. i. *)
+(*             rewrite <- View.join_assoc. *)
+(*             etrans; [|apply View.join_l]. *)
+(*             eapply future_stable_view; try eapply GET; try eapply join_stable_view; eauto. *)
+(*             * eapply Memory.join_closed_view; ss. *)
+(*               { inv CLOSED_RELEASEDM; ss. *)
+(*                 apply Memory.closed_view_bot. apply MEM1. } *)
+(*               { apply WF1. } *)
+(*             * apply STABLE_TVIEW1. ss. *)
+(*       } *)
+
+(*       i. des. splits; auto. *)
+(*       ii. exploit RELS_WF1; eauto. i. des. *)
+(*       exploit Memory.promise_get1; try exact x0; eauto; try by (inv PROMISE; ss). i. des. inv MSG_LE. *)
+(*       esplits; eauto. s. *)
+(*       erewrite Memory.remove_o; eauto. condtac; ss. guardH o. *)
+(*       inv PROMISE; ss. *)
+(*       - erewrite Memory.add_o; eauto. condtac; ss. *)
+(*       - erewrite Memory.split_o; eauto. repeat condtac; ss. *)
+(*         guardH o0. des. subst. *)
+(*         exploit Memory.split_get0; try exact PROMISES. i. des. congr. *)
+(*       - erewrite Memory.lower_o; eauto. condtac; ss. *)
+(*     Qed. *)
+
+(*     Lemma write_step_other_None *)
+(*           rels lc1 sc1 mem1 loc from to val released ord lc2 sc2 mem2 kind *)
+(*           (WF1: Local.wf lc1 mem1) *)
+(*           (SC1: Memory.closed_timemap sc1 mem1) *)
+(*           (MEM1: Memory.closed mem1) *)
+(*           (NORMAL_TVIEW1: normal_tview (Local.tview lc1)) *)
+(*           (NORMAL_MEM1: normal_memory mem1) *)
+(*           (STABLE_TVIEW1: stable_tview mem1 (Local.tview lc1)) *)
+(*           (STABLE_MEM1: stable_memory rels mem1) *)
+(*           (RELS_WF1: RelWrites.wf rels (Local.promises lc1) mem1) *)
+(*           (LOC: ~ L loc) *)
+(*           (STEP: Local.write_step lc1 sc1 mem1 loc from to val None released ord lc2 sc2 mem2 kind): *)
+(*       <<NORMAL_TVIEW2: normal_tview (Local.tview lc2)>> /\ *)
+(*       <<NORMAL_MEM2: normal_memory mem2>> /\ *)
+(*       <<STABLE_TVIEW2: stable_tview mem2 (Local.tview lc2)>> /\ *)
+(*       <<STABLE_MEM2: stable_memory rels mem2>> /\ *)
+(*       <<RELS_WF2: RelWrites.wf rels (Local.promises lc2) mem2>>. *)
+(*     Proof. *)
+(*       eapply write_step_other; eauto; ss. *)
+(*       apply bot_stable_view. apply MEM1. *)
+(*     Qed. *)
+
+(*     Lemma fence_step *)
+(*           rels lc1 sc1 mem1 ordr ordw lc2 sc2 *)
+(*           (WF1: Local.wf lc1 mem1) *)
+(*           (NORMAL_TVIEW1: normal_tview (Local.tview lc1)) *)
+(*           (STABLE_TVIEW1: stable_tview mem1 (Local.tview lc1)) *)
+(*           (STABLE_SC1: stable_timemap mem1 sc1) *)
+(*           (RELS_WF1: RelWrites.wf rels (Local.promises lc1) mem1) *)
+(*           (STEP: Local.fence_step lc1 sc1 ordr ordw lc2 sc2): *)
+(*       <<NORMAL_TVIEW2: normal_tview (Local.tview lc2)>> /\ *)
+(*       <<STABLE_TVIEW2: stable_tview mem1 (Local.tview lc2)>> /\ *)
+(*       <<STABLE_SC2: stable_timemap mem1 sc2>> /\ *)
+(*       <<RELS_WF2: RelWrites.wf rels (Local.promises lc2) mem1>>. *)
+(*     Proof. *)
+(*       inv STEP. ss. splits; ss. *)
+(*       - inv NORMAL_TVIEW1. *)
+(*         econs; ss; i; repeat (condtac; ss). *)
+(*         + apply join_normal_view; ss. *)
+(*         + apply join_normal_view; ss. *)
+(*       - inv STABLE_TVIEW1. *)
+(*         econs; ss; i; repeat (condtac; ss); eauto. *)
+(*         + unfold TView.write_fence_sc. repeat (condtac; ss). *)
+(*           * hexploit join_stable_view; [apply STABLE_SC1| apply ACQ|]. i. *)
+(*             unfold View.join in H. ss. ii. *)
+(*             etrans; [eapply H; eauto|]. *)
+(*             econs; try refl. ss. *)
+(*             apply TimeMap.join_spec. *)
+(*             { apply TimeMap.join_l. } *)
+(*             { etrans; [|apply TimeMap.join_r]. apply WF1. } *)
+(*           * hexploit join_stable_view; [apply STABLE_SC1| apply CUR|]. i. *)
+(*             unfold View.join in H. ss. ii. *)
+(*             etrans; [eapply H; eauto|]. *)
+(*             econs; try refl. ss. *)
+(*             apply TimeMap.join_spec. *)
+(*             { apply TimeMap.join_l. } *)
+(*             { etrans; [|apply TimeMap.join_r]. apply WF1. } *)
+(*         + unfold TView.write_fence_sc. repeat (condtac; ss). *)
+(*           * hexploit join_stable_view; [apply STABLE_SC1| apply ACQ|]. i. *)
+(*             unfold View.join in H. ss. ii. *)
+(*             etrans; [eapply H; eauto|]. *)
+(*             econs; try refl. ss. *)
+(*             apply TimeMap.join_spec. *)
+(*             { apply TimeMap.join_l. } *)
+(*             { etrans; [|apply TimeMap.join_r]. apply WF1. } *)
+(*           * hexploit join_stable_view; [apply STABLE_SC1| apply CUR|]. i. *)
+(*             unfold View.join in H. ss. ii. *)
+(*             etrans; [eapply H; eauto|]. *)
+(*             econs; try refl. ss. *)
+(*             apply TimeMap.join_spec. *)
+(*             { apply TimeMap.join_l. } *)
+(*             { etrans; [|apply TimeMap.join_r]. apply WF1. } *)
+(*         + unfold TView.write_fence_sc. repeat (condtac; ss). *)
+(*           * apply join_stable_view; ss. *)
+(*             hexploit join_stable_view; [apply STABLE_SC1| apply ACQ|]. i. *)
+(*             unfold View.join in H. ss. ii. *)
+(*             etrans; [eapply H; eauto|]. *)
+(*             econs; try refl. ss. *)
+(*             apply TimeMap.join_spec. *)
+(*             { apply TimeMap.join_l. } *)
+(*             { etrans; [|apply TimeMap.join_r]. apply WF1. } *)
+(*           * apply join_stable_view; ss. *)
+(*             hexploit join_stable_view; [apply STABLE_SC1| apply CUR|]. i. *)
+(*             unfold View.join in H. ss. ii. *)
+(*             etrans; [eapply H; eauto|]. *)
+(*             econs; try refl. ss. *)
+(*             apply TimeMap.join_spec. *)
+(*             { apply TimeMap.join_l. } *)
+(*             { etrans; [|apply TimeMap.join_r]. apply WF1. } *)
+(*         + rewrite View.le_join_l; try by apply View.bot_spec. ss. *)
+(*       - unfold TView.write_fence_sc. repeat (condtac; ss). *)
+(*         + eapply join_stable_timemap; ss. *)
+(*           apply stable_view_stable_timemap. *)
+(*           * apply WF1. *)
+(*           * apply STABLE_TVIEW1. *)
+(*         + eapply join_stable_timemap; ss. *)
+(*           apply stable_view_stable_timemap. *)
+(*           * apply WF1. *)
+(*           * apply STABLE_TVIEW1. *)
+(*     Qed. *)
+
+
+(*     (* cap *) *)
+
+(*     Lemma max_concrete_timemap_stable *)
+(*           mem tm *)
+(*           (CLOSED: Memory.closed mem) *)
+(*           (MAX: Memory.max_concrete_timemap mem tm): *)
+(*       stable_timemap mem tm. *)
+(*     Proof. *)
+(*       ii. dup CLOSED. inv CLOSED. *)
+(*       exploit CLOSED1; eauto. i. des. inv MSG_CLOSED. inv CLOSED. inv CLOSED2. *)
+(*       hexploit Memory.max_concrete_timemap_spec; try exact PLN; eauto. i. *)
+(*       hexploit Memory.max_concrete_timemap_spec; try exact RLX; eauto. i. *)
+(*       econs; ss. *)
+(*     Qed. *)
+
+(*     Lemma cap_normal_memory *)
+(*           mem1 mem2 *)
+(*           (CLOSED: Memory.closed mem1) *)
+(*           (CAP: Memory.cap mem1 mem2) *)
+(*           (NORMAL: normal_memory mem1): *)
+(*       normal_memory mem2. *)
+(*     Proof. *)
+(*       ii. exploit Memory.cap_inv; eauto. i. des; ss. *)
+(*       eapply NORMAL; eauto. *)
+(*     Qed. *)
+
+(*     Lemma cap_stable_view *)
+(*           mem1 mem2 view *)
+(*           (CLOSED: Memory.closed mem1) *)
+(*           (CAP: Memory.cap mem1 mem2) *)
+(*           (STABLE: stable_view mem1 view): *)
+(*       stable_view mem2 view. *)
+(*     Proof. *)
+(*       ii. exploit Memory.cap_inv; eauto. i. des; ss. *)
+(*       eapply STABLE; eauto. *)
+(*     Qed. *)
+
+(*     Lemma cap_stable_timemap *)
+(*           mem1 mem2 tm *)
+(*           (CLOSED: Memory.closed mem1) *)
+(*           (CAP: Memory.cap mem1 mem2) *)
+(*           (STABLE: stable_timemap mem1 tm): *)
+(*       stable_timemap mem2 tm. *)
+(*     Proof. *)
+(*       eapply cap_stable_view; eauto. *)
+(*     Qed. *)
+
+(*     Lemma cap_stable_tview *)
+(*           mem1 mem2 tview *)
+(*           (CLOSED: Memory.closed mem1) *)
+(*           (CAP: Memory.cap mem1 mem2) *)
+(*           (STABLE: stable_tview mem1 tview): *)
+(*       stable_tview mem2 tview. *)
+(*     Proof. *)
+(*       inv STABLE. econs; eauto using cap_stable_view. *)
+(*     Qed. *)
+
+(*     Lemma cap_stable_memory *)
+(*           rels mem1 mem2 *)
+(*           (CLOSED: Memory.closed mem1) *)
+(*           (CAP: Memory.cap mem1 mem2) *)
+(*           (STABLE: stable_memory rels mem1): *)
+(*       stable_memory rels mem2. *)
+(*     Proof. *)
+(*       ii. guardH LOC. *)
+(*       exploit Memory.cap_inv; try exact GET; eauto. i. des; ss. *)
+(*       exploit Memory.cap_inv; try exact GET0; eauto. i. des; ss. *)
+(*       eapply STABLE; eauto. *)
+(*     Qed. *)
+(*   End Stable. *)
+(* End Stable. *)
